Add lemma, update patterns for EDTL

EDTL_Patterns.thy
@@ -16,7 +16,7 @@ consecutive s0 s \<Longrightarrow>
 EDTL_delay_true_inv w_0 trigger fin release_1 Inv_1 reaction_1 s"
 
 unfolding EDTL_delay_true_inv_def
-apply(erule always_rule)
+apply(erule always_inv_saving_gen)
   apply simp
   apply(erule conjE)
   subgoal premises prems1
@@ -38,7 +38,7 @@ apply(erule always_rule)
           apply(insert prems3(1,2))[1]
             apply simp
           apply(insert prems3(1,3))
-            apply(rule weak_until_rule)
+            apply(rule weak_until_L1)
             apply simp
               apply(erule conjE)
               subgoal premises prems4
@@ -142,7 +142,7 @@ apply(erule always_rule)
       apply(rule disjI1)
         apply simp
       apply(rule disjI2)
-        apply(rule weak_until_one_point)
+        apply(rule weak_until_L2)
         apply simp
           apply(erule disjE)
           apply(rule disjI1)
@@ -191,7 +191,7 @@ toEnvP s0 \<Longrightarrow>
 EDTL_delay_true trigger fin release Inv reaction s0"
 
 unfolding EDTL_delay_true_inv_def EDTL_delay_true_def
-apply(erule always_einv2req)
+apply(erule always_einv_imp_req_gen)
 apply simp
   apply(rule always_disj_rule)
   apply simp
@@ -209,7 +209,7 @@ apply simp
         apply(insert prems4(1,2))[1]
           apply simp
         apply(insert prems4(1,3))
-          apply(rule weak_until_einv2req)
+          apply(rule weak_until_L3)
           apply simp
             apply(erule conjE)
             subgoal premises prems5
@@ -309,7 +309,7 @@ apply(erule conjE)
 subgoal premises prems1
 apply(rule conjI)
 apply(insert prems1(1,2,4))[1]
-apply(erule always_rule)
+apply(erule always_inv_saving_gen)
   apply simp
   apply(erule conjE)
   subgoal premises prems2
@@ -321,7 +321,7 @@ apply(erule always_rule)
       subgoal premises prems3
       apply(rule conjI)
       apply(insert prems3(1,2))[1]
-        apply(rule weak_previous_LS4)
+        apply(rule weak_previous_L4)
         apply simp
           apply(rule always_imp_refl)
       apply(insert prems3(1,3))
@@ -333,7 +333,7 @@ apply(erule always_rule)
           apply(insert prems4(1,2))[1]
             apply simp
           apply(insert prems4(1,3))
-            apply(rule weak_until_rule)
+            apply(rule weak_until_L1)
             apply simp
               apply(erule conjE)
               subgoal premises prems5
@@ -431,7 +431,7 @@ apply(erule always_rule)
   apply(insert prems2(1,3))
     apply(erule disjE)
     apply(rule disjI1)
-      apply(rule weak_previous_one_point[OF prems1(3)])
+      apply(rule weak_previous_L7[OF prems1(3)])
       apply simp
         apply(erule conjE)
         subgoal premises prems15
@@ -446,7 +446,7 @@ apply(erule always_rule)
       apply(rule disjI1)
         apply simp
       apply(rule disjI2)
-        apply(rule weak_until_one_point)
+        apply(rule weak_until_L2)
         apply simp
           apply(erule disjE)
           apply(rule disjI1)
@@ -487,7 +487,7 @@ apply(erule always_rule)
             done
   done
 apply(insert prems1(1,3,5))
-  apply(erule previous_rule)
+  apply(erule previous_inv_L6)
   apply simp
   apply(rule impI)
   apply(erule impE)
@@ -511,7 +511,7 @@ apply(insert prems1(1,2))
 apply(erule conjE)
 subgoal premises prems2
 apply(insert prems2(1,2) prems1(3))
-apply(erule always_einv2req)
+apply(erule always_einv_imp_req_gen)
 apply simp
   apply(rule always_disj_rule)
   apply simp
@@ -519,7 +519,7 @@ apply simp
     subgoal premises prems3
     apply(rule conjI)
     apply(insert prems3(1,2))[1]
-      apply(rule weak_previous_LS5)
+      apply(rule weak_previous_L5)
       apply simp
         apply(rule always_imp_refl)
     apply(insert prems3(1,3))
@@ -531,7 +531,7 @@ apply simp
         apply(insert prems4(1,2))[1]
           apply simp
         apply(insert prems4(1,3))
-          apply(rule weak_until_einv2req)
+          apply(rule weak_until_L3)
           apply simp
             apply(erule conjE)
             subgoal premises prems5
@@ -613,493 +613,6 @@ lemmas EDTL_trigger_prev_delay_true_inv_part_used_patterns = EDTL_trigger_prev_d
 
 lemmas EDTL_trigger_prev_delay_true_part_used_patterns = EDTL_trigger_prev_delay_true_part_def EDTL_trigger_prev_delay_true_used_patterns
 
-definition EDTL_final_nontemporal_or_tau_delay_true where "EDTL_final_nontemporal_or_tau_delay_true finalt trigger finale release Inv reaction s \<equiv> (always (\<lambda> r2 r1 . ((\<not> (trigger r1)) \<or> ((release r2 r1) \<or> ((constrained_until finalt (\<lambda> r4 r3 . ((Inv r4 r3) \<and> (\<not> (finale r3)))) (\<lambda> r4 r3 . ((release r4 r3) \<or> ((finale r3) \<and> ((reaction r4 r3) \<and> (Inv r4 r3))))) r2 r1) \<or> (constrained_until2 finalt finalt (\<lambda> r4 r3 . ((Inv r4 r3) \<and> (\<not> (finale r3)))) (\<lambda> r4 r3 . ((reaction r4 r3) \<and> (Inv r4 r3))) r2 r1))))) s)"
-
-definition EDTL_final_nontemporal_or_tau_delay_true_part where "EDTL_final_nontemporal_or_tau_delay_true_part finalt trigger finale release Inv reaction s \<equiv> (EDTL_final_nontemporal_or_tau_delay_true finalt trigger finale (\<lambda> s s1 . (release s1)) (\<lambda> s s1 . (Inv s1)) (\<lambda> s s1 . (reaction s1)) s)"
-
-definition EDTL_final_nontemporal_or_tau_delay_true_inv where "EDTL_final_nontemporal_or_tau_delay_true_inv finalt t1_0 t1_1_0 t2_1_0 trigger finale release_1 Inv_1 reaction_1 s \<equiv> (always_inv (\<lambda> r2 r1 . ((\<not> (trigger r1)) \<or> ((release_1 r2 r1) \<or> ((constrained_until_inv finalt t1_0 (\<lambda> r4 r3 . ((Inv_1 r4 r3) \<and> (\<not> (finale r3)))) (\<lambda> r4 r3 . ((release_1 r4 r3) \<or> ((finale r3) \<and> ((reaction_1 r4 r3) \<and> (Inv_1 r4 r3))))) r2 r1) \<or> (constrained_until2_inv finalt finalt t1_1_0 t2_1_0 (\<lambda> r4 r3 . ((Inv_1 r4 r3) \<and> (\<not> (finale r3)))) (\<lambda> r4 r3 . ((reaction_1 r4 r3) \<and> (Inv_1 r4 r3))) r2 r1))))) s)"
-
-definition EDTL_final_nontemporal_or_tau_delay_true_inv_part where "EDTL_final_nontemporal_or_tau_delay_true_inv_part finalt t1_0 t1_1_0 t2_1_0 trigger finale release Inv reaction s \<equiv> (EDTL_final_nontemporal_or_tau_delay_true_inv finalt t1_0 t1_1_0 t2_1_0 trigger finale (\<lambda> s s1 . (release s1)) (\<lambda> s s1 . (Inv s1)) (\<lambda> s s1 . (reaction s1)) s)"
-
-lemma EDTL_final_nontemporal_or_tau_delay_true_inv_saving_gen: "
-EDTL_final_nontemporal_or_tau_delay_true_inv finalt t1_0 t1_1_0 t2_1_0 trigger finale release_1 Inv_1 reaction_1 s0 \<Longrightarrow>
-consecutive s0 s \<Longrightarrow>
-((True \<and> ((always_imp s0 (\<lambda> r1 . (release_1 s0 r1)) (\<lambda> r1 . (release_1 s r1))) \<and> ((((always_imp s0 (\<lambda> r3 . (Inv_1 s0 r3)) (\<lambda> r3 . (Inv_1 s r3))) \<and> True) \<and> (((always_imp s0 (\<lambda> r3 . (release_1 s0 r3)) (\<lambda> r3 . (release_1 s r3))) \<and> (True \<and> ((always_imp s0 (\<lambda> r3 . (reaction_1 s0 r3)) (\<lambda> r3 . (reaction_1 s r3))) \<and> (always_imp s0 (\<lambda> r3 . (Inv_1 s0 r3)) (\<lambda> r3 . (Inv_1 s r3)))))) \<and> (((t1_0 s0) = 0) \<or> ((((release_1 s s) \<or> ((finale s) \<and> ((reaction_1 s s) \<and> (Inv_1 s s)))) \<and> ((t1_0 s0) <= finalt)) \<or> (((Inv_1 s s) \<and> (\<not> (finale s))) \<and> ((t1_0 s0) < (t1_0 s))))))) \<and> (((always_imp s0 (\<lambda> r3 . (Inv_1 s0 r3)) (\<lambda> r3 . (Inv_1 s r3))) \<and> True) \<and> (((always_imp s0 (\<lambda> r3 . (reaction_1 s0 r3)) (\<lambda> r3 . (reaction_1 s r3))) \<and> (always_imp s0 (\<lambda> r3 . (Inv_1 s0 r3)) (\<lambda> r3 . (Inv_1 s r3)))) \<and> (((t2_1_0 s0) = 0) \<or> (((t1_1_0 s0) >= (t2_1_0 s0)) \<or> ((((reaction_1 s s) \<and> (Inv_1 s s)) \<and> ((((t1_1_0 s0) + 1) >= finalt) \<and> ((t2_1_0 s0) <= finalt))) \<or> (((Inv_1 s s) \<and> (\<not> (finale s))) \<and> ((((t1_1_0 s0) + 1) >= (t1_1_0 s)) \<and> ((t2_1_0 s0) < (t2_1_0 s)))))))))))) \<and> ((\<not> (trigger s)) \<or> ((release_1 s s) \<or> ((((release_1 s s) \<or> ((finale s) \<and> ((reaction_1 s s) \<and> (Inv_1 s s)))) \<or> (((Inv_1 s s) \<and> (\<not> (finale s))) \<and> ((t1_0 s) > 0))) \<or> (((finalt = 0) \<and> ((reaction_1 s s) \<and> (Inv_1 s s))) \<or> (((Inv_1 s s) \<and> (\<not> (finale s))) \<and> (((t1_1_0 s) = 0) \<and> ((t2_1_0 s) > 0)))))))) \<Longrightarrow>
-EDTL_final_nontemporal_or_tau_delay_true_inv finalt t1_0 t1_1_0 t2_1_0 trigger finale release_1 Inv_1 reaction_1 s"
-
-unfolding EDTL_final_nontemporal_or_tau_delay_true_inv_def
-apply(erule always_rule)
-  apply simp
-  apply(erule conjE)
-  subgoal premises prems1
-  apply(rule conjI)
-  apply(insert prems1(1,2))[1]
-    apply(rule always_disj_rule)
-    apply simp
-      apply(erule conjE)
-      subgoal premises prems2
-      apply(rule conjI)
-      apply(insert prems2(1,2))[1]
-        apply(rule always_imp_refl)
-      apply(insert prems2(1,3))
-        apply(rule always_disj_rule)
-        apply simp
-          apply(erule conjE)
-          subgoal premises prems3
-          apply(rule conjI)
-          apply(insert prems3(1,2))[1]
-            apply simp
-          apply(insert prems3(1,3))
-            apply(rule always_disj_rule)
-            apply simp
-              apply(erule conjE)
-              subgoal premises prems4
-              apply(rule conjI)
-              apply(insert prems4(1,2))[1]
-                apply(rule constrained_until_rule)
-                apply simp
-                  apply(erule conjE)
-                  subgoal premises prems5
-                  apply(rule conjI)
-                  apply(insert prems5(1,2))[1]
-                    apply(rule always_conj_rule)
-                    apply simp
-                      apply(erule conjE)
-                      subgoal premises prems6
-                      apply(rule conjI)
-                      apply(insert prems6(1,2))[1]
-                        apply simp
-                      apply(insert prems6(1,3))
-                        apply(rule always_imp_refl)
-                      done
-                  apply(insert prems5(1,3))
-                    apply(erule conjE)
-                    subgoal premises prems7
-                    apply(rule conjI)
-                    apply(insert prems7(1,2))[1]
-                      apply(rule always_disj_rule)
-                      apply simp
-                        apply(erule conjE)
-                        subgoal premises prems8
-                        apply(rule conjI)
-                        apply(insert prems8(1,2))[1]
-                          apply simp
-                        apply(insert prems8(1,3))
-                          apply(rule always_conj_rule)
-                          apply simp
-                            apply(erule conjE)
-                            subgoal premises prems9
-                            apply(rule conjI)
-                            apply(insert prems9(1,2))[1]
-                              apply(rule always_imp_refl)
-                            apply(insert prems9(1,3))
-                              apply(rule always_conj_rule)
-                              apply simp
-                                apply(erule conjE)
-                                subgoal premises prems10
-                                apply(rule conjI)
-                                apply(insert prems10(1,2))[1]
-                                  apply simp
-                                apply(insert prems10(1,3))
-                                  apply simp
-                                done
-                            done
-                        done
-                    apply(insert prems7(1,3))
-                      apply(erule disjE)
-                      apply(rule disjI1)
-                        apply simp
-                      apply(rule disjI2)
-                        apply(erule disjE)
-                        apply(rule disjI1)
-                          apply(erule conjE)
-                          subgoal premises prems11
-                          apply(rule conjI)
-                          apply(insert prems11(1,2))[1]
-                            apply(erule disjE)
-                            apply(rule disjI1)
-                              apply simp
-                            apply(rule disjI2)
-                              apply(erule conjE)
-                              subgoal premises prems12
-                              apply(rule conjI)
-                              apply(insert prems12(1,2))[1]
-                                apply simp
-                              apply(insert prems12(1,3))
-                                apply(erule conjE)
-                                subgoal premises prems13
-                                apply(rule conjI)
-                                apply(insert prems13(1,2))[1]
-                                  apply simp
-                                apply(insert prems13(1,3))
-                                  apply simp
-                                done
-                              done
-                          apply(insert prems11(1,3))
-                            apply simp
-                          done
-                        apply(rule disjI2)
-                          apply(erule conjE)
-                          subgoal premises prems14
-                          apply(rule conjI)
-                          apply(insert prems14(1,2))[1]
-                            apply(erule conjE)
-                            subgoal premises prems15
-                            apply(rule conjI)
-                            apply(insert prems15(1,2))[1]
-                              apply simp
-                            apply(insert prems15(1,3))
-                              apply simp
-                            done
-                          apply(insert prems14(1,3))
-                            apply simp
-                          done
-                    done
-                  done
-              apply(insert prems4(1,3))
-                apply(rule constrained_until2_rule)
-                apply simp
-                  apply(erule conjE)
-                  subgoal premises prems16
-                  apply(rule conjI)
-                  apply(insert prems16(1,2))[1]
-                    apply(rule always_conj_rule)
-                    apply simp
-                      apply(erule conjE)
-                      subgoal premises prems17
-                      apply(rule conjI)
-                      apply(insert prems17(1,2))[1]
-                        apply simp
-                      apply(insert prems17(1,3))
-                        apply(rule always_imp_refl)
-                      done
-                  apply(insert prems16(1,3))
-                    apply(erule conjE)
-                    subgoal premises prems18
-                    apply(rule conjI)
-                    apply(insert prems18(1,2))[1]
-                      apply(rule always_conj_rule)
-                      apply simp
-                        apply(erule conjE)
-                        subgoal premises prems19
-                        apply(rule conjI)
-                        apply(insert prems19(1,2))[1]
-                          apply simp
-                        apply(insert prems19(1,3))
-                          apply simp
-                        done
-                    apply(insert prems18(1,3))
-                      apply(erule disjE)
-                      apply(rule disjI1)
-                        apply simp
-                      apply(rule disjI2)
-                        apply(erule disjE)
-                        apply(rule disjI1)
-                          apply simp
-                        apply(rule disjI2)
-                          apply(erule disjE)
-                          apply(rule disjI1)
-                            apply(erule conjE)
-                            subgoal premises prems20
-                            apply(rule conjI)
-                            apply(insert prems20(1,2))[1]
-                              apply(erule conjE)
-                              subgoal premises prems21
-                              apply(rule conjI)
-                              apply(insert prems21(1,2))[1]
-                                apply simp
-                              apply(insert prems21(1,3))
-                                apply simp
-                              done
-                            apply(insert prems20(1,3))
-                              apply(erule conjE)
-                              subgoal premises prems22
-                              apply(rule conjI)
-                              apply(insert prems22(1,2))[1]
-                                apply simp
-                              apply(insert prems22(1,3))
-                                apply simp
-                              done
-                            done
-                          apply(rule disjI2)
-                            apply(erule conjE)
-                            subgoal premises prems23
-                            apply(rule conjI)
-                            apply(insert prems23(1,2))[1]
-                              apply(erule conjE)
-                              subgoal premises prems24
-                              apply(rule conjI)
-                              apply(insert prems24(1,2))[1]
-                                apply simp
-                              apply(insert prems24(1,3))
-                                apply simp
-                              done
-                            apply(insert prems23(1,3))
-                              apply(erule conjE)
-                              subgoal premises prems25
-                              apply(rule conjI)
-                              apply(insert prems25(1,2))[1]
-                                apply simp
-                              apply(insert prems25(1,3))
-                                apply simp
-                              done
-                            done
-                    done
-                  done
-              done
-          done
-      done
-  apply(insert prems1(1,3))
-    apply(erule disjE)
-    apply(rule disjI1)
-      apply simp
-    apply(rule disjI2)
-      apply(erule disjE)
-      apply(rule disjI1)
-        apply simp
-      apply(rule disjI2)
-        apply(erule disjE)
-        apply(rule disjI1)
-          apply(rule constrained_until_one_point)
-          apply simp
-            apply(erule disjE)
-            apply(rule disjI1)
-              apply(erule disjE)
-              apply(rule disjI1)
-                apply simp
-              apply(rule disjI2)
-                apply(erule conjE)
-                subgoal premises prems26
-                apply(rule conjI)
-                apply(insert prems26(1,2))[1]
-                  apply simp
-                apply(insert prems26(1,3))
-                  apply(erule conjE)
-                  subgoal premises prems27
-                  apply(rule conjI)
-                  apply(insert prems27(1,2))[1]
-                    apply simp
-                  apply(insert prems27(1,3))
-                    apply simp
-                  done
-                done
-            apply(rule disjI2)
-              apply(erule conjE)
-              subgoal premises prems28
-              apply(rule conjI)
-              apply(insert prems28(1,2))[1]
-                apply(erule conjE)
-                subgoal premises prems29
-                apply(rule conjI)
-                apply(insert prems29(1,2))[1]
-                  apply simp
-                apply(insert prems29(1,3))
-                  apply simp
-                done
-              apply(insert prems28(1,3))
-                apply simp
-              done
-        apply(rule disjI2)
-          apply(rule constrained_until2_one_point)
-          apply simp
-            apply(erule disjE)
-            apply(rule disjI1)
-              apply(erule conjE)
-              subgoal premises prems30
-              apply(rule conjI)
-              apply(insert prems30(1,2))[1]
-                apply simp
-              apply(insert prems30(1,3))
-                apply(erule conjE)
-                subgoal premises prems31
-                apply(rule conjI)
-                apply(insert prems31(1,2))[1]
-                  apply simp
-                apply(insert prems31(1,3))
-                  apply simp
-                done
-              done
-            apply(rule disjI2)
-              apply(erule conjE)
-              subgoal premises prems32
-              apply(rule conjI)
-              apply(insert prems32(1,2))[1]
-                apply(erule conjE)
-                subgoal premises prems33
-                apply(rule conjI)
-                apply(insert prems33(1,2))[1]
-                  apply simp
-                apply(insert prems33(1,3))
-                  apply simp
-                done
-              apply(insert prems32(1,3))
-                apply(erule conjE)
-                subgoal premises prems34
-                apply(rule conjI)
-                apply(insert prems34(1,2))[1]
-                  apply simp
-                apply(insert prems34(1,3))
-                  apply simp
-                done
-              done
-  done
-done
-
-lemma EDTL_final_nontemporal_or_tau_delay_trueeinv_imp_req_gen: "
-EDTL_final_nontemporal_or_tau_delay_true_inv finalt t1_0 t1_1_0 t2_1_0 trigger finale release_1 Inv_1 reaction_1 s0 \<Longrightarrow>
-toEnvP s0 \<Longrightarrow>
-(True \<and> ((always_imp s0 (\<lambda> r1 . (release_1 s0 r1)) (\<lambda> r1 . (release s0 r1))) \<and> ((((always_imp s0 (\<lambda> r3 . (Inv_1 s0 r3)) (\<lambda> r3 . (Inv s0 r3))) \<and> True) \<and> (((always_imp s0 (\<lambda> r3 . (release_1 s0 r3)) (\<lambda> r3 . (release s0 r3))) \<and> (True \<and> ((always_imp s0 (\<lambda> r3 . (reaction_1 s0 r3)) (\<lambda> r3 . (reaction s0 r3))) \<and> (always_imp s0 (\<lambda> r3 . (Inv_1 s0 r3)) (\<lambda> r3 . (Inv s0 r3)))))) \<and> ((t1_0 s0) <= finalt))) \<and> (((always_imp s0 (\<lambda> r3 . (Inv_1 s0 r3)) (\<lambda> r3 . (Inv s0 r3))) \<and> True) \<and> (((always_imp s0 (\<lambda> r3 . (reaction_1 s0 r3)) (\<lambda> r3 . (reaction s0 r3))) \<and> (always_imp s0 (\<lambda> r3 . (Inv_1 s0 r3)) (\<lambda> r3 . (Inv s0 r3)))) \<and> ((t2_1_0 s0) <= finalt)))))) \<Longrightarrow>
-EDTL_final_nontemporal_or_tau_delay_true finalt trigger finale release Inv reaction s0"
-
-unfolding EDTL_final_nontemporal_or_tau_delay_true_inv_def EDTL_final_nontemporal_or_tau_delay_true_def
-apply(erule always_einv2req)
-apply simp
-  apply(rule always_disj_rule)
-  apply simp
-    apply(erule conjE)
-    subgoal premises prems3
-    apply(rule conjI)
-    apply(insert prems3(1,2))[1]
-      apply(rule always_imp_refl)
-    apply(insert prems3(1,3))
-      apply(rule always_disj_rule)
-      apply simp
-        apply(erule conjE)
-        subgoal premises prems4
-        apply(rule conjI)
-        apply(insert prems4(1,2))[1]
-          apply simp
-        apply(insert prems4(1,3))
-          apply(rule always_disj_rule)
-          apply simp
-            apply(erule conjE)
-            subgoal premises prems5
-            apply(rule conjI)
-            apply(insert prems5(1,2))[1]
-              apply(rule constrained_until_einv2req)
-              apply simp
-                apply(erule conjE)
-                subgoal premises prems6
-                apply(rule conjI)
-                apply(insert prems6(1,2))[1]
-                  apply(rule always_conj_rule)
-                  apply simp
-                    apply(erule conjE)
-                    subgoal premises prems7
-                    apply(rule conjI)
-                    apply(insert prems7(1,2))[1]
-                      apply simp
-                    apply(insert prems7(1,3))
-                      apply(rule always_imp_refl)
-                    done
-                apply(insert prems6(1,3))
-                  apply(erule conjE)
-                  subgoal premises prems8
-                  apply(rule conjI)
-                  apply(insert prems8(1,2))[1]
-                    apply(rule always_disj_rule)
-                    apply simp
-                      apply(erule conjE)
-                      subgoal premises prems9
-                      apply(rule conjI)
-                      apply(insert prems9(1,2))[1]
-                        apply simp
-                      apply(insert prems9(1,3))
-                        apply(rule always_conj_rule)
-                        apply simp
-                          apply(erule conjE)
-                          subgoal premises prems10
-                          apply(rule conjI)
-                          apply(insert prems10(1,2))[1]
-                            apply(rule always_imp_refl)
-                          apply(insert prems10(1,3))
-                            apply(rule always_conj_rule)
-                            apply simp
-                              apply(erule conjE)
-                              subgoal premises prems11
-                              apply(rule conjI)
-                              apply(insert prems11(1,2))[1]
-                                apply simp
-                              apply(insert prems11(1,3))
-                                apply simp
-                              done
-                          done
-                      done
-                  apply(insert prems8(1,3))
-                    apply simp
-                  done
-                done
-            apply(insert prems5(1,3))
-              apply(rule constrained_until2_einv2req)
-              apply simp
-                apply(erule conjE)
-                subgoal premises prems12
-                apply(rule conjI)
-                apply(insert prems12(1,2))[1]
-                  apply(rule always_conj_rule)
-                  apply simp
-                    apply(erule conjE)
-                    subgoal premises prems13
-                    apply(rule conjI)
-                    apply(insert prems13(1,2))[1]
-                      apply simp
-                    apply(insert prems13(1,3))
-                      apply(rule always_imp_refl)
-                    done
-                apply(insert prems12(1,3))
-                  apply(erule conjE)
-                  subgoal premises prems14
-                  apply(rule conjI)
-                  apply(insert prems14(1,2))[1]
-                    apply(rule always_conj_rule)
-                    apply simp
-                      apply(erule conjE)
-                      subgoal premises prems15
-                      apply(rule conjI)
-                      apply(insert prems15(1,2))[1]
-                        apply simp
-                      apply(insert prems15(1,3))
-                        apply simp
-                      done
-                  apply(insert prems14(1,3))
-                    apply simp
-                  done
-                done
-            done
-        done
-    done
-done
-
-lemma EDTL_final_nontemporal_or_tau_delay_true_inv_saving: "
-EDTL_final_nontemporal_or_tau_delay_true_inv_part finalt t1_0 t1_1_0 t2_1_0 trigger finale release Inv reaction s0 \<Longrightarrow>
-consecutive s0 s \<Longrightarrow>
-(((((t1_0 s0) = 0) \<or> ((((release s) \<or> ((finale s) \<and> ((reaction s) \<and> (Inv s)))) \<and> ((t1_0 s0) <= finalt)) \<or> (((Inv s) \<and> (\<not> (finale s))) \<and> ((t1_0 s0) < (t1_0 s))))) \<and> (((t2_1_0 s0) = 0) \<or> (((t1_1_0 s0) >= (t2_1_0 s0)) \<or> ((((reaction s) \<and> (Inv s)) \<and> ((((t1_1_0 s0) + 1) >= finalt) \<and> ((t2_1_0 s0) <= finalt))) \<or> (((Inv s) \<and> (\<not> (finale s))) \<and> ((((t1_1_0 s0) + 1) >= (t1_1_0 s)) \<and> ((t2_1_0 s0) < (t2_1_0 s)))))))) \<and> ((\<not> (trigger s)) \<or> ((release s) \<or> ((((release s) \<or> ((finale s) \<and> ((reaction s) \<and> (Inv s)))) \<or> (((Inv s) \<and> (\<not> (finale s))) \<and> ((t1_0 s) > 0))) \<or> (((finalt = 0) \<and> ((reaction s) \<and> (Inv s))) \<or> (((Inv s) \<and> (\<not> (finale s))) \<and> (((t1_1_0 s) = 0) \<and> ((t2_1_0 s) > 0)))))))) \<Longrightarrow>
-EDTL_final_nontemporal_or_tau_delay_true_inv_part finalt t1_0 t1_1_0 t2_1_0 trigger finale release Inv reaction s"
-
-unfolding EDTL_final_nontemporal_or_tau_delay_true_inv_part_def EDTL_final_nontemporal_or_tau_delay_true_part_def
-apply(simp add: EDTL_final_nontemporal_or_tau_delay_true_inv_saving_gen always_imp_refl)
-done
-
-lemma EDTL_final_nontemporal_or_tau_delay_trueeinv_imp_req: "
-EDTL_final_nontemporal_or_tau_delay_true_inv_part finalt t1_0 t1_1_0 t2_1_0 trigger finale release Inv reaction s \<Longrightarrow>
-toEnvP s \<Longrightarrow>
-(((t1_0 s) <= finalt) \<and> ((t2_1_0 s) <= finalt)) \<Longrightarrow>
-EDTL_final_nontemporal_or_tau_delay_true_part finalt trigger finale release Inv reaction s"
-
-unfolding EDTL_final_nontemporal_or_tau_delay_true_inv_part_def EDTL_final_nontemporal_or_tau_delay_true_part_def
-apply(simp add: EDTL_final_nontemporal_or_tau_delay_trueeinv_imp_req_gen always_imp_refl)
-done
-
-
-
-lemmas EDTL_final_nontemporal_or_tau_delay_true_used_patterns = EDTL_final_nontemporal_or_tau_delay_true_def always_used_patterns constrained_until_def constrained_until2_def 
-
-lemmas EDTL_final_nontemporal_or_tau_delay_true_inv_used_patterns = EDTL_final_nontemporal_or_tau_delay_true_inv_def always_inv_used_patterns constrained_until_inv_def constrained_until2_inv_def 
-
-lemmas EDTL_final_nontemporal_or_tau_delay_true_inv_part_used_patterns = EDTL_final_nontemporal_or_tau_delay_true_inv_part_def EDTL_final_nontemporal_or_tau_delay_true_inv_used_patterns
-
-lemmas EDTL_final_nontemporal_or_tau_delay_true_part_used_patterns = EDTL_final_nontemporal_or_tau_delay_true_part_def EDTL_final_nontemporal_or_tau_delay_true_used_patterns
-
 definition EDTL_final_prev_delay_true where "EDTL_final_prev_delay_true trigger fin release Inv reaction s \<equiv> (always (\<lambda> r2 r1 . ((\<not> (trigger r1)) \<or> ((release r2 r1) \<or> (weak_until (\<lambda> r4 r3 . ((Inv r4 r3) \<and> (weak_previous (\<lambda> r6 r5 . (\<not> (fin r5))) r4 r3))) (\<lambda> r4 r3 . ((release r4 r3) \<or> ((previous (\<lambda> r6 r5 . (fin r5)) r4 r3) \<and> ((reaction r4 r3) \<and> (Inv r4 r3))))) r2 r1)))) s)"
 
 definition EDTL_final_prev_delay_true_part where "EDTL_final_prev_delay_true_part trigger fin release Inv reaction s \<equiv> (EDTL_final_prev_delay_true trigger fin (\<lambda> s s1 . (release s1)) (\<lambda> s s1 . (Inv s1)) (\<lambda> s s1 . (reaction s1)) s)"
@@ -1125,7 +638,7 @@ apply(erule conjE)
 subgoal premises prems2
 apply(rule conjI)
 apply(insert prems2(1,2,4))[1]
-apply(erule always_rule)
+apply(erule always_inv_saving_gen)
   apply simp
   apply(erule conjE)
   subgoal premises prems3
@@ -1147,7 +660,7 @@ apply(erule always_rule)
           apply(insert prems5(1,2))[1]
             apply simp
           apply(insert prems5(1,3))
-            apply(rule weak_until_rule)
+            apply(rule weak_until_L1)
             apply simp
               apply(erule conjE)
               subgoal premises prems6
@@ -1161,7 +674,7 @@ apply(erule always_rule)
                   apply(insert prems7(1,2))[1]
                     apply simp
                   apply(insert prems7(1,3))
-                    apply(rule weak_previous_LS4)
+                    apply(rule weak_previous_L4)
                     apply simp
                       apply(rule always_imp_refl)
                   done
@@ -1184,7 +697,7 @@ apply(erule always_rule)
                         subgoal premises prems10
                         apply(rule conjI)
                         apply(insert prems10(1,2))[1]
-                          apply(rule previous_LS4)
+                          apply(rule previous_L4)
                           apply simp
                             apply(rule always_imp_refl)
                         apply(insert prems10(1,3))
@@ -1215,7 +728,7 @@ apply(erule always_rule)
                         subgoal premises prems12
                         apply(rule conjI)
                         apply(insert prems12(1,2))[1]
-                          apply(rule previous_one_point[OF prems1(3)])
+                          apply(rule previous_L7[OF prems1(3)])
                           apply simp
                             apply(erule conjE)
                             subgoal premises prems13
@@ -1248,7 +761,7 @@ apply(erule always_rule)
                         apply(insert prems16(1,2))[1]
                           apply simp
                         apply(insert prems16(1,3))
-                          apply(rule weak_previous_one_point[OF prems2(3)])
+                          apply(rule weak_previous_L7[OF prems2(3)])
                           apply simp
                             apply(erule conjE)
                             subgoal premises prems17
@@ -1273,7 +786,7 @@ apply(erule always_rule)
       apply(rule disjI1)
         apply simp
       apply(rule disjI2)
-        apply(rule weak_until_one_point)
+        apply(rule weak_until_L2)
         apply simp
           apply(erule disjE)
           apply(rule disjI1)
@@ -1285,7 +798,7 @@ apply(erule always_rule)
               subgoal premises prems18
               apply(rule conjI)
               apply(insert prems18(1,2))[1]
-                apply(rule previous_one_point[OF prems1(3)])
+                apply(rule previous_L7[OF prems1(3)])
                 apply simp
                   apply(erule conjE)
                   subgoal premises prems19
@@ -1318,7 +831,7 @@ apply(erule always_rule)
               apply(insert prems22(1,2))[1]
                 apply simp
               apply(insert prems22(1,3))
-                apply(rule weak_previous_one_point[OF prems2(3)])
+                apply(rule weak_previous_L7[OF prems2(3)])
                 apply simp
                   apply(erule conjE)
                   subgoal premises prems23
@@ -1332,7 +845,7 @@ apply(erule always_rule)
             done
   done
 apply(insert prems2(1,3,5))
-  apply(erule previous_rule)
+  apply(erule previous_inv_L6)
   apply simp
   apply(rule impI)
   apply(erule impE)
@@ -1343,7 +856,7 @@ apply(insert prems2(1,3,5))
   done
 done
 apply(insert prems1(1,3,5))
-  apply(erule previous_rule)
+  apply(erule previous_inv_L6)
   apply simp
   apply(rule impI)
   apply(erule impE)
@@ -1368,7 +881,7 @@ apply(simp only: conj_assoc)
 apply(erule conjE)
 subgoal premises prems2
 apply(insert prems2(1,2) prems1(3))
-apply(erule always_einv2req)
+apply(erule always_einv_imp_req_gen)
 apply simp
   apply(rule always_disj_rule)
   apply simp
@@ -1386,7 +899,7 @@ apply simp
         apply(insert prems4(1,2))[1]
           apply simp
         apply(insert prems4(1,3))
-          apply(rule weak_until_einv2req)
+          apply(rule weak_until_L3)
           apply simp
             apply(erule conjE)
             subgoal premises prems5
@@ -1400,7 +913,7 @@ apply simp
                 apply(insert prems6(1,2))[1]
                   apply simp
                 apply(insert prems6(1,3))
-                  apply(rule weak_previous_LS5)
+                  apply(rule weak_previous_L5)
                   apply simp
                     apply(rule always_imp_refl)
                 done
@@ -1419,7 +932,7 @@ apply simp
                     subgoal premises prems8
                     apply(rule conjI)
                     apply(insert prems8(1,2))[1]
-                      apply(rule previous_LS5)
+                      apply(rule previous_L5)
                       apply simp
                         apply(rule always_imp_refl)
                     apply(insert prems8(1,3))
@@ -1502,7 +1015,7 @@ apply(erule conjE)
 subgoal premises prems3
 apply(rule conjI)
 apply(insert prems3(1,2,4))[1]
-apply(erule always_rule)
+apply(erule always_inv_saving_gen)
   apply simp
   apply(erule conjE)
   subgoal premises prems4
@@ -1514,7 +1027,7 @@ apply(erule always_rule)
       subgoal premises prems5
       apply(rule conjI)
       apply(insert prems5(1,2))[1]
-        apply(rule weak_previous_LS4)
+        apply(rule weak_previous_L4)
         apply simp
           apply(rule always_imp_refl)
       apply(insert prems5(1,3))
@@ -1526,7 +1039,7 @@ apply(erule always_rule)
           apply(insert prems6(1,2))[1]
             apply simp
           apply(insert prems6(1,3))
-            apply(rule weak_until_rule)
+            apply(rule weak_until_L1)
             apply simp
               apply(erule conjE)
               subgoal premises prems7
@@ -1540,7 +1053,7 @@ apply(erule always_rule)
                   apply(insert prems8(1,2))[1]
                     apply simp
                   apply(insert prems8(1,3))
-                    apply(rule weak_previous_LS4)
+                    apply(rule weak_previous_L4)
                     apply simp
                       apply(rule always_imp_refl)
                   done
@@ -1563,7 +1076,7 @@ apply(erule always_rule)
                         subgoal premises prems11
                         apply(rule conjI)
                         apply(insert prems11(1,2))[1]
-                          apply(rule previous_LS4)
+                          apply(rule previous_L4)
                           apply simp
                             apply(rule always_imp_refl)
                         apply(insert prems11(1,3))
@@ -1594,7 +1107,7 @@ apply(erule always_rule)
                         subgoal premises prems13
                         apply(rule conjI)
                         apply(insert prems13(1,2))[1]
-                          apply(rule previous_one_point[OF prems1(3)])
+                          apply(rule previous_L7[OF prems1(3)])
                           apply simp
                             apply(erule conjE)
                             subgoal premises prems14
@@ -1627,7 +1140,7 @@ apply(erule always_rule)
                         apply(insert prems17(1,2))[1]
                           apply simp
                         apply(insert prems17(1,3))
-                          apply(rule weak_previous_one_point[OF prems2(3)])
+                          apply(rule weak_previous_L7[OF prems2(3)])
                           apply simp
                             apply(erule conjE)
                             subgoal premises prems18
@@ -1646,7 +1159,7 @@ apply(erule always_rule)
   apply(insert prems4(1,3))
     apply(erule disjE)
     apply(rule disjI1)
-      apply(rule weak_previous_one_point[OF prems3(3)])
+      apply(rule weak_previous_L7[OF prems3(3)])
       apply simp
         apply(erule conjE)
         subgoal premises prems19
@@ -1661,7 +1174,7 @@ apply(erule always_rule)
       apply(rule disjI1)
         apply simp
       apply(rule disjI2)
-        apply(rule weak_until_one_point)
+        apply(rule weak_until_L2)
         apply simp
           apply(erule disjE)
           apply(rule disjI1)
@@ -1673,7 +1186,7 @@ apply(erule always_rule)
               subgoal premises prems20
               apply(rule conjI)
               apply(insert prems20(1,2))[1]
-                apply(rule previous_one_point[OF prems1(3)])
+                apply(rule previous_L7[OF prems1(3)])
                 apply simp
                   apply(erule conjE)
                   subgoal premises prems21
@@ -1706,7 +1219,7 @@ apply(erule always_rule)
               apply(insert prems24(1,2))[1]
                 apply simp
               apply(insert prems24(1,3))
-                apply(rule weak_previous_one_point[OF prems2(3)])
+                apply(rule weak_previous_L7[OF prems2(3)])
                 apply simp
                   apply(erule conjE)
                   subgoal premises prems25
@@ -1720,7 +1233,7 @@ apply(erule always_rule)
             done
   done
 apply(insert prems3(1,3,5))
-  apply(erule previous_rule)
+  apply(erule previous_inv_L6)
   apply simp
   apply(rule impI)
   apply(erule impE)
@@ -1731,7 +1244,7 @@ apply(insert prems3(1,3,5))
   done
 done
 apply(insert prems2(1,3,5))
-  apply(erule previous_rule)
+  apply(erule previous_inv_L6)
   apply simp
   apply(rule impI)
   apply(erule impE)
@@ -1742,7 +1255,7 @@ apply(insert prems2(1,3,5))
   done
 done
 apply(insert prems1(1,3,5))
-  apply(erule previous_rule)
+  apply(erule previous_inv_L6)
   apply simp
   apply(rule impI)
   apply(erule impE)
@@ -1767,7 +1280,7 @@ apply(simp only: conj_assoc)
 apply(erule conjE)
 subgoal premises prems2
 apply(insert prems2(1,2) prems1(3))
-apply(erule always_einv2req)
+apply(erule always_einv_imp_req_gen)
 apply simp
   apply(rule always_disj_rule)
   apply simp
@@ -1775,7 +1288,7 @@ apply simp
     subgoal premises prems3
     apply(rule conjI)
     apply(insert prems3(1,2))[1]
-      apply(rule weak_previous_LS5)
+      apply(rule weak_previous_L5)
       apply simp
         apply(rule always_imp_refl)
     apply(insert prems3(1,3))
@@ -1787,7 +1300,7 @@ apply simp
         apply(insert prems4(1,2))[1]
           apply simp
         apply(insert prems4(1,3))
-          apply(rule weak_until_einv2req)
+          apply(rule weak_until_L3)
           apply simp
             apply(erule conjE)
             subgoal premises prems5
@@ -1801,7 +1314,7 @@ apply simp
                 apply(insert prems6(1,2))[1]
                   apply simp
                 apply(insert prems6(1,3))
-                  apply(rule weak_previous_LS5)
+                  apply(rule weak_previous_L5)
                   apply simp
                     apply(rule always_imp_refl)
                 done
@@ -1820,7 +1333,7 @@ apply simp
                     subgoal premises prems8
                     apply(rule conjI)
                     apply(insert prems8(1,2))[1]
-                      apply(rule previous_LS5)
+                      apply(rule previous_L5)
                       apply simp
                         apply(rule always_imp_refl)
                     apply(insert prems8(1,3))
@@ -1873,110 +1386,106 @@ lemmas EDTL_trigger_prev_final_prev_delay_true_inv_part_used_patterns = EDTL_tri
 
 lemmas EDTL_trigger_prev_final_prev_delay_true_part_used_patterns = EDTL_trigger_prev_final_prev_delay_true_part_def EDTL_trigger_prev_final_prev_delay_true_used_patterns
 
-definition EDTL_trigger_prev_final_nontemporal_or_tau_delay_true where "EDTL_trigger_prev_final_nontemporal_or_tau_delay_true finalt trigger finale release Inv reaction s \<equiv> (always (\<lambda> r2 r1 . ((weak_previous (\<lambda> r4 r3 . (\<not> (trigger r3))) r2 r1) \<or> ((release r2 r1) \<or> ((constrained_until finalt (\<lambda> r4 r3 . ((Inv r4 r3) \<and> (\<not> (finale r3)))) (\<lambda> r4 r3 . ((release r4 r3) \<or> ((finale r3) \<and> ((reaction r4 r3) \<and> (Inv r4 r3))))) r2 r1) \<or> (constrained_until2 finalt finalt (\<lambda> r4 r3 . ((Inv r4 r3) \<and> (\<not> (finale r3)))) (\<lambda> r4 r3 . ((reaction r4 r3) \<and> (Inv r4 r3))) r2 r1))))) s)"
+definition EDTL_final_nontemporal_or_tau_delay_true where "EDTL_final_nontemporal_or_tau_delay_true finalt trigger finale release Inv reaction s \<equiv> ((always (\<lambda> r2 r1 . ((\<not> (trigger r1)) \<or> ((release r2 r1) \<or> (constrained_weak_until (finalt + 1) (\<lambda> r4 r3 . ((Inv r4 r3) \<and> (\<not> (finale r3)))) (\<lambda> r4 r3 . ((release r4 r3) \<or> ((finale r3) \<and> ((reaction r4 r3) \<and> (Inv r4 r3))))) r2 r1)))) s) \<and>(always (\<lambda> r2 r1 . ((dual_constrained_since finalt finalt (\<lambda> r4 r3 . (finale r3)) (\<lambda> r4 r3 . ((\<not> (trigger r3)) \<or> (finale r3))) r2 r1) \<or> (reaction r2 r1))) s))"
 
-definition EDTL_trigger_prev_final_nontemporal_or_tau_delay_true_part where "EDTL_trigger_prev_final_nontemporal_or_tau_delay_true_part finalt trigger finale release Inv reaction s \<equiv> (EDTL_trigger_prev_final_nontemporal_or_tau_delay_true finalt trigger finale (\<lambda> s s1 . (release s1)) (\<lambda> s s1 . (Inv s1)) (\<lambda> s s1 . (reaction s1)) s)"
+definition EDTL_final_nontemporal_or_tau_delay_true_part where "EDTL_final_nontemporal_or_tau_delay_true_part finalt trigger finale release Inv reaction s \<equiv> (EDTL_final_nontemporal_or_tau_delay_true finalt trigger finale (\<lambda> s s1 . (release s1)) (\<lambda> s s1 . (Inv s1)) (\<lambda> s s1 . (reaction s1)) s)"
 
-definition EDTL_trigger_prev_final_nontemporal_or_tau_delay_true_inv where "EDTL_trigger_prev_final_nontemporal_or_tau_delay_true_inv finalt b_0 t1_0 t1_1_0 t2_1_0 trigger finale release_1 Inv_1 reaction_1 s \<equiv> ((always_inv (\<lambda> r2 r1 . ((weak_previous (\<lambda> r4 r3 . (\<not> (trigger r3))) r2 r1) \<or> ((release_1 r2 r1) \<or> ((constrained_until_inv finalt t1_0 (\<lambda> r4 r3 . ((Inv_1 r4 r3) \<and> (\<not> (finale r3)))) (\<lambda> r4 r3 . ((release_1 r4 r3) \<or> ((finale r3) \<and> ((reaction_1 r4 r3) \<and> (Inv_1 r4 r3))))) r2 r1) \<or> (constrained_until2_inv finalt finalt t1_1_0 t2_1_0 (\<lambda> r4 r3 . ((Inv_1 r4 r3) \<and> (\<not> (finale r3)))) (\<lambda> r4 r3 . ((reaction_1 r4 r3) \<and> (Inv_1 r4 r3))) r2 r1))))) s) \<and> (previous_inv b_0 (\<lambda> r4 r3 . (\<not> (trigger r3))) s))"
+definition EDTL_final_nontemporal_or_tau_delay_true_inv where "EDTL_final_nontemporal_or_tau_delay_true_inv finalt t1_0 b_0 t1_1_0 t2_1_0 trigger finale release_1 Inv_1 reaction_1 s \<equiv> ((always_inv (\<lambda> r2 r1 . ((\<not> (trigger r1)) \<or> ((release_1 r2 r1) \<or> (constrained_weak_until_inv (finalt + 1) t1_0 (\<lambda> r4 r3 . ((Inv_1 r4 r3) \<and> (\<not> (finale r3)))) (\<lambda> r4 r3 . ((release_1 r4 r3) \<or> ((finale r3) \<and> ((reaction_1 r4 r3) \<and> (Inv_1 r4 r3))))) r2 r1)))) s) \<and> ((always_inv (\<lambda> r2 r1 . ((dual_constrained_since finalt finalt (\<lambda> r4 r3 . (finale r3)) (\<lambda> r4 r3 . ((\<not> (trigger r3)) \<or> (finale r3))) r2 r1) \<or> (reaction_1 r2 r1))) s) \<and> (dual_constrained_since_inv finalt finalt b_0 t1_1_0 t2_1_0 (\<lambda> r4 r3 . (finale r3)) (\<lambda> r4 r3 . ((\<not> (trigger r3)) \<or> (finale r3))) s)))"
 
-definition EDTL_trigger_prev_final_nontemporal_or_tau_delay_true_inv_part where "EDTL_trigger_prev_final_nontemporal_or_tau_delay_true_inv_part finalt b_0 t1_0 t1_1_0 t2_1_0 trigger finale release Inv reaction s \<equiv> (EDTL_trigger_prev_final_nontemporal_or_tau_delay_true_inv finalt b_0 t1_0 t1_1_0 t2_1_0 trigger finale (\<lambda> s s1 . (release s1)) (\<lambda> s s1 . (Inv s1)) (\<lambda> s s1 . (reaction s1)) s)"
+definition EDTL_final_nontemporal_or_tau_delay_true_inv_part where "EDTL_final_nontemporal_or_tau_delay_true_inv_part finalt t1_0 b_0 t1_1_0 t2_1_0 trigger finale release Inv reaction s \<equiv> (EDTL_final_nontemporal_or_tau_delay_true_inv finalt t1_0 b_0 t1_1_0 t2_1_0 trigger finale (\<lambda> s s1 . (release s1)) (\<lambda> s s1 . (Inv s1)) (\<lambda> s s1 . (reaction s1)) s)"
 
-lemma EDTL_trigger_prev_final_nontemporal_or_tau_delay_true_inv_saving_gen: "
-EDTL_trigger_prev_final_nontemporal_or_tau_delay_true_inv finalt b_0 t1_0 t1_1_0 t2_1_0 trigger finale release_1 Inv_1 reaction_1 s0 \<Longrightarrow>
+lemma EDTL_final_nontemporal_or_tau_delay_true_inv_saving_gen: "
+EDTL_final_nontemporal_or_tau_delay_true_inv finalt t1_0 b_0 t1_1_0 t2_1_0 trigger finale release_1 Inv_1 reaction_1 s0 \<Longrightarrow>
 consecutive s0 s \<Longrightarrow>
-(((True \<and> ((always_imp s0 (\<lambda> r1 . (release_1 s0 r1)) (\<lambda> r1 . (release_1 s r1))) \<and> ((((always_imp s0 (\<lambda> r3 . (Inv_1 s0 r3)) (\<lambda> r3 . (Inv_1 s r3))) \<and> True) \<and> (((always_imp s0 (\<lambda> r3 . (release_1 s0 r3)) (\<lambda> r3 . (release_1 s r3))) \<and> (True \<and> ((always_imp s0 (\<lambda> r3 . (reaction_1 s0 r3)) (\<lambda> r3 . (reaction_1 s r3))) \<and> (always_imp s0 (\<lambda> r3 . (Inv_1 s0 r3)) (\<lambda> r3 . (Inv_1 s r3)))))) \<and> (((t1_0 s0) = 0) \<or> ((((release_1 s s) \<or> ((finale s) \<and> ((reaction_1 s s) \<and> (Inv_1 s s)))) \<and> ((t1_0 s0) <= finalt)) \<or> (((Inv_1 s s) \<and> (\<not> (finale s))) \<and> ((t1_0 s0) < (t1_0 s))))))) \<and> (((always_imp s0 (\<lambda> r3 . (Inv_1 s0 r3)) (\<lambda> r3 . (Inv_1 s r3))) \<and> True) \<and> (((always_imp s0 (\<lambda> r3 . (reaction_1 s0 r3)) (\<lambda> r3 . (reaction_1 s r3))) \<and> (always_imp s0 (\<lambda> r3 . (Inv_1 s0 r3)) (\<lambda> r3 . (Inv_1 s r3)))) \<and> (((t2_1_0 s0) = 0) \<or> (((t1_1_0 s0) >= (t2_1_0 s0)) \<or> ((((reaction_1 s s) \<and> (Inv_1 s s)) \<and> ((((t1_1_0 s0) + 1) >= finalt) \<and> ((t2_1_0 s0) <= finalt))) \<or> (((Inv_1 s s) \<and> (\<not> (finale s))) \<and> ((((t1_1_0 s0) + 1) >= (t1_1_0 s)) \<and> ((t2_1_0 s0) < (t2_1_0 s)))))))))))) \<and> (((b_0 s0) \<and> True) \<or> ((release_1 s s) \<or> ((((release_1 s s) \<or> ((finale s) \<and> ((reaction_1 s s) \<and> (Inv_1 s s)))) \<or> (((Inv_1 s s) \<and> (\<not> (finale s))) \<and> ((t1_0 s) > 0))) \<or> (((finalt = 0) \<and> ((reaction_1 s s) \<and> (Inv_1 s s))) \<or> (((Inv_1 s s) \<and> (\<not> (finale s))) \<and> (((t1_1_0 s) = 0) \<and> ((t2_1_0 s) > 0)))))))) \<and> ((b_0 s) --> (\<not> (trigger s)))) \<Longrightarrow>
-EDTL_trigger_prev_final_nontemporal_or_tau_delay_true_inv finalt b_0 t1_0 t1_1_0 t2_1_0 trigger finale release_1 Inv_1 reaction_1 s"
+(((True \<and> ((always_imp s0 (\<lambda> r1 . (release_1 s0 r1)) (\<lambda> r1 . (release_1 s r1))) \<and> (((always_imp s0 (\<lambda> r3 . (Inv_1 s0 r3)) (\<lambda> r3 . (Inv_1 s r3))) \<and> True) \<and> (((always_imp s0 (\<lambda> r3 . (release_1 s0 r3)) (\<lambda> r3 . (release_1 s r3))) \<and> (True \<and> ((always_imp s0 (\<lambda> r3 . (reaction_1 s0 r3)) (\<lambda> r3 . (reaction_1 s r3))) \<and> (always_imp s0 (\<lambda> r3 . (Inv_1 s0 r3)) (\<lambda> r3 . (Inv_1 s r3)))))) \<and> ((((t1_0 s0) < (finalt + 1)) \<and> ((((release_1 s s) \<or> ((finale s) \<and> ((reaction_1 s s) \<and> (Inv_1 s s)))) \<and> ((t1_0 s) <= ((finalt + 1) + 1))) \<or> (((t1_0 s) <= ((t1_0 s0) + 1)) \<and> ((Inv_1 s s) \<and> (\<not> (finale s)))))) \<or> (((t1_0 s0) >= (finalt + 1)) \<and> ((t1_0 s) <= ((t1_0 s0) + 1)))))))) \<and> ((\<not> (trigger s)) \<or> ((release_1 s s) \<or> (((release_1 s s) \<or> ((finale s) \<and> ((reaction_1 s s) \<and> (Inv_1 s s)))) \<or> (((t1_0 s) = 0) \<and> ((Inv_1 s s) \<and> (\<not> (finale s)))))))) \<and> ((((True \<and> True) \<and> (always_imp s0 (\<lambda> r1 . (reaction_1 s0 r1)) (\<lambda> r1 . (reaction_1 s r1)))) \<and> ((((finalt > 0) \<or> ((\<not> (trigger s)) \<or> (finale s))) \<and> ((finale s) \<or> ((b_0 s0) \<and> (True \<and> (True \<and> (((t1_1_0 s0) < finalt) \<and> (finalt <= ((t2_1_0 s0) + 1)))))))) \<or> (reaction_1 s s))) \<and> ((b_0 s) --> ((((t1_1_0 s) > 0) \<or> ((\<not> (trigger s)) \<or> (finale s))) \<and> ((finale s) \<or> ((b_0 s0) \<and> (True \<and> (True \<and> (((t1_1_0 s0) < (t1_1_0 s)) \<and> ((t2_1_0 s) <= ((t2_1_0 s0) + 1))))))))))) \<Longrightarrow>
+EDTL_final_nontemporal_or_tau_delay_true_inv finalt t1_0 b_0 t1_1_0 t2_1_0 trigger finale release_1 Inv_1 reaction_1 s"
 
-unfolding EDTL_trigger_prev_final_nontemporal_or_tau_delay_true_inv_def
+unfolding EDTL_final_nontemporal_or_tau_delay_true_inv_def
 apply(erule conjE)
 apply(erule conjE)
 subgoal premises prems1
 apply(rule conjI)
 apply(insert prems1(1,2,4))[1]
-apply(erule always_rule)
-  apply simp
-  apply(erule conjE)
-  subgoal premises prems2
-  apply(rule conjI)
-  apply(insert prems2(1,2))[1]
-    apply(rule always_disj_rule)
+  apply(erule always_inv_saving_gen)
     apply simp
-      apply(erule conjE)
-      subgoal premises prems3
-      apply(rule conjI)
-      apply(insert prems3(1,2))[1]
-        apply(rule weak_previous_LS4)
-        apply simp
+    apply(erule conjE)
+    subgoal premises prems2
+    apply(rule conjI)
+    apply(insert prems2(1,2))[1]
+      apply(rule always_disj_rule)
+      apply simp
+        apply(erule conjE)
+        subgoal premises prems3
+        apply(rule conjI)
+        apply(insert prems3(1,2))[1]
           apply(rule always_imp_refl)
-      apply(insert prems3(1,3))
-        apply(rule always_disj_rule)
-        apply simp
-          apply(erule conjE)
-          subgoal premises prems4
-          apply(rule conjI)
-          apply(insert prems4(1,2))[1]
-            apply simp
-          apply(insert prems4(1,3))
-            apply(rule always_disj_rule)
-            apply simp
-              apply(erule conjE)
-              subgoal premises prems5
-              apply(rule conjI)
-              apply(insert prems5(1,2))[1]
-                apply(rule constrained_until_rule)
-                apply simp
+        apply(insert prems3(1,3))
+          apply(rule always_disj_rule)
+          apply simp
+            apply(erule conjE)
+            subgoal premises prems4
+            apply(rule conjI)
+            apply(insert prems4(1,2))[1]
+              apply simp
+            apply(insert prems4(1,3))
+              apply(rule constrained_weak_until_L1)
+              apply simp
+                apply(erule conjE)
+                subgoal premises prems5
+                apply(rule conjI)
+                apply(insert prems5(1,2))[1]
+                  apply(rule always_conj_rule)
+                  apply simp
+                    apply(erule conjE)
+                    subgoal premises prems6
+                    apply(rule conjI)
+                    apply(insert prems6(1,2))[1]
+                      apply simp
+                    apply(insert prems6(1,3))
+                      apply(rule always_imp_refl)
+                    done
+                apply(insert prems5(1,3))
                   apply(erule conjE)
-                  subgoal premises prems6
+                  subgoal premises prems7
                   apply(rule conjI)
-                  apply(insert prems6(1,2))[1]
-                    apply(rule always_conj_rule)
+                  apply(insert prems7(1,2))[1]
+                    apply(rule always_disj_rule)
                     apply simp
                       apply(erule conjE)
-                      subgoal premises prems7
+                      subgoal premises prems8
                       apply(rule conjI)
-                      apply(insert prems7(1,2))[1]
+                      apply(insert prems8(1,2))[1]
                         apply simp
-                      apply(insert prems7(1,3))
-                        apply(rule always_imp_refl)
+                      apply(insert prems8(1,3))
+                        apply(rule always_conj_rule)
+                        apply simp
+                          apply(erule conjE)
+                          subgoal premises prems9
+                          apply(rule conjI)
+                          apply(insert prems9(1,2))[1]
+                            apply(rule always_imp_refl)
+                          apply(insert prems9(1,3))
+                            apply(rule always_conj_rule)
+                            apply simp
+                              apply(erule conjE)
+                              subgoal premises prems10
+                              apply(rule conjI)
+                              apply(insert prems10(1,2))[1]
+                                apply simp
+                              apply(insert prems10(1,3))
+                                apply simp
+                              done
+                          done
                       done
-                  apply(insert prems6(1,3))
-                    apply(erule conjE)
-                    subgoal premises prems8
-                    apply(rule conjI)
-                    apply(insert prems8(1,2))[1]
-                      apply(rule always_disj_rule)
-                      apply simp
-                        apply(erule conjE)
-                        subgoal premises prems9
-                        apply(rule conjI)
-                        apply(insert prems9(1,2))[1]
-                          apply simp
-                        apply(insert prems9(1,3))
-                          apply(rule always_conj_rule)
-                          apply simp
-                            apply(erule conjE)
-                            subgoal premises prems10
-                            apply(rule conjI)
-                            apply(insert prems10(1,2))[1]
-                              apply(rule always_imp_refl)
-                            apply(insert prems10(1,3))
-                              apply(rule always_conj_rule)
-                              apply simp
-                                apply(erule conjE)
-                                subgoal premises prems11
-                                apply(rule conjI)
-                                apply(insert prems11(1,2))[1]
-                                  apply simp
-                                apply(insert prems11(1,3))
-                                  apply simp
-                                done
-                            done
-                        done
-                    apply(insert prems8(1,3))
-                      apply(erule disjE)
-                      apply(rule disjI1)
+                  apply(insert prems7(1,3))
+                    apply(erule disjE)
+                    apply(rule disjI1)
+                      apply(erule conjE)
+                      subgoal premises prems11
+                      apply(rule conjI)
+                      apply(insert prems11(1,2))[1]
                         apply simp
-                      apply(rule disjI2)
+                      apply(insert prems11(1,3))
                         apply(erule disjE)
                         apply(rule disjI1)
                           apply(erule conjE)
@@ -2010,6 +1519,8 @@ apply(erule always_rule)
                           subgoal premises prems15
                           apply(rule conjI)
                           apply(insert prems15(1,2))[1]
+                            apply simp
+                          apply(insert prems15(1,3))
                             apply(erule conjE)
                             subgoal premises prems16
                             apply(rule conjI)
@@ -2018,125 +1529,24 @@ apply(erule always_rule)
                             apply(insert prems16(1,3))
                               apply simp
                             done
-                          apply(insert prems15(1,3))
-                            apply simp
                           done
-                    done
-                  done
-              apply(insert prems5(1,3))
-                apply(rule constrained_until2_rule)
-                apply simp
-                  apply(erule conjE)
-                  subgoal premises prems17
-                  apply(rule conjI)
-                  apply(insert prems17(1,2))[1]
-                    apply(rule always_conj_rule)
-                    apply simp
-                      apply(erule conjE)
-                      subgoal premises prems18
-                      apply(rule conjI)
-                      apply(insert prems18(1,2))[1]
-                        apply simp
-                      apply(insert prems18(1,3))
-                        apply(rule always_imp_refl)
                       done
-                  apply(insert prems17(1,3))
-                    apply(erule conjE)
-                    subgoal premises prems19
-                    apply(rule conjI)
-                    apply(insert prems19(1,2))[1]
-                      apply(rule always_conj_rule)
+                    apply(rule disjI2)
                       apply simp
-                        apply(erule conjE)
-                        subgoal premises prems20
-                        apply(rule conjI)
-                        apply(insert prems20(1,2))[1]
-                          apply simp
-                        apply(insert prems20(1,3))
-                          apply simp
-                        done
-                    apply(insert prems19(1,3))
-                      apply(erule disjE)
-                      apply(rule disjI1)
-                        apply simp
-                      apply(rule disjI2)
-                        apply(erule disjE)
-                        apply(rule disjI1)
-                          apply simp
-                        apply(rule disjI2)
-                          apply(erule disjE)
-                          apply(rule disjI1)
-                            apply(erule conjE)
-                            subgoal premises prems21
-                            apply(rule conjI)
-                            apply(insert prems21(1,2))[1]
-                              apply(erule conjE)
-                              subgoal premises prems22
-                              apply(rule conjI)
-                              apply(insert prems22(1,2))[1]
-                                apply simp
-                              apply(insert prems22(1,3))
-                                apply simp
-                              done
-                            apply(insert prems21(1,3))
-                              apply(erule conjE)
-                              subgoal premises prems23
-                              apply(rule conjI)
-                              apply(insert prems23(1,2))[1]
-                                apply simp
-                              apply(insert prems23(1,3))
-                                apply simp
-                              done
-                            done
-                          apply(rule disjI2)
-                            apply(erule conjE)
-                            subgoal premises prems24
-                            apply(rule conjI)
-                            apply(insert prems24(1,2))[1]
-                              apply(erule conjE)
-                              subgoal premises prems25
-                              apply(rule conjI)
-                              apply(insert prems25(1,2))[1]
-                                apply simp
-                              apply(insert prems25(1,3))
-                                apply simp
-                              done
-                            apply(insert prems24(1,3))
-                              apply(erule conjE)
-                              subgoal premises prems26
-                              apply(rule conjI)
-                              apply(insert prems26(1,2))[1]
-                                apply simp
-                              apply(insert prems26(1,3))
-                                apply simp
-                              done
-                            done
-                    done
                   done
-              done
-          done
-      done
-  apply(insert prems2(1,3))
-    apply(erule disjE)
-    apply(rule disjI1)
-      apply(rule weak_previous_one_point[OF prems1(3)])
-      apply simp
-        apply(erule conjE)
-        subgoal premises prems27
-        apply(rule conjI)
-        apply(insert prems27(1,2))[1]
-          apply simp
-        apply(insert prems27(1,3))
-          apply(rule always_imp_refl)
+                done
+            done
         done
-    apply(rule disjI2)
+    apply(insert prems2(1,3))
       apply(erule disjE)
       apply(rule disjI1)
         apply simp
       apply(rule disjI2)
         apply(erule disjE)
         apply(rule disjI1)
-          apply(rule constrained_until_one_point)
+          apply simp
+        apply(rule disjI2)
+          apply(rule constrained_weak_until_L2)
           apply simp
             apply(erule disjE)
             apply(rule disjI1)
@@ -2145,124 +1555,351 @@ apply(erule always_rule)
                 apply simp
               apply(rule disjI2)
                 apply(erule conjE)
-                subgoal premises prems28
+                subgoal premises prems17
                 apply(rule conjI)
-                apply(insert prems28(1,2))[1]
+                apply(insert prems17(1,2))[1]
                   apply simp
-                apply(insert prems28(1,3))
+                apply(insert prems17(1,3))
                   apply(erule conjE)
-                  subgoal premises prems29
+                  subgoal premises prems18
                   apply(rule conjI)
-                  apply(insert prems29(1,2))[1]
+                  apply(insert prems18(1,2))[1]
                     apply simp
-                  apply(insert prems29(1,3))
+                  apply(insert prems18(1,3))
                     apply simp
                   done
                 done
             apply(rule disjI2)
               apply(erule conjE)
-              subgoal premises prems30
+              subgoal premises prems19
               apply(rule conjI)
-              apply(insert prems30(1,2))[1]
+              apply(insert prems19(1,2))[1]
+                apply simp
+              apply(insert prems19(1,3))
                 apply(erule conjE)
-                subgoal premises prems31
+                subgoal premises prems20
                 apply(rule conjI)
-                apply(insert prems31(1,2))[1]
+                apply(insert prems20(1,2))[1]
                   apply simp
-                apply(insert prems31(1,3))
+                apply(insert prems20(1,3))
                   apply simp
                 done
-              apply(insert prems30(1,3))
-                apply simp
               done
-        apply(rule disjI2)
-          apply(rule constrained_until2_one_point)
+    done
+apply(insert prems1(1,3,5))
+  apply(erule conjE)
+  apply(erule conjE)
+  subgoal premises prems21
+  apply(rule conjI)
+  apply(insert prems21(1,2,4))[1]
+  apply(erule always_inv_saving_gen)
+    apply simp
+    apply(erule conjE)
+    subgoal premises prems22
+    apply(rule conjI)
+    apply(insert prems22(1,2))[1]
+      apply(rule always_disj_rule)
+      apply simp
+        apply(erule conjE)
+        subgoal premises prems23
+        apply(rule conjI)
+        apply(insert prems23(1,2))[1]
+          apply(rule dual_constrained_since_L4)
           apply simp
+            apply(erule conjE)
+            subgoal premises prems24
+            apply(rule conjI)
+            apply(insert prems24(1,2))[1]
+              apply(rule always_imp_refl)
+            apply(insert prems24(1,3))
+              apply(rule always_imp_refl)
+            done
+        apply(insert prems23(1,3))
+          apply simp
+        done
+    apply(insert prems22(1,3))
+      apply(erule disjE)
+      apply(rule disjI1)
+        apply(rule dual_constrained_since_L7[OF prems21(3)])
+        apply simp
+          apply(erule conjE)
+          subgoal premises prems25
+          apply(rule conjI)
+          apply(insert prems25(1,2))[1]
             apply(erule disjE)
             apply(rule disjI1)
-              apply(erule conjE)
-              subgoal premises prems32
-              apply(rule conjI)
-              apply(insert prems32(1,2))[1]
+              apply simp
+            apply(rule disjI2)
+              apply(erule disjE)
+              apply(rule disjI1)
                 apply simp
-              apply(insert prems32(1,3))
-                apply(erule conjE)
-                subgoal premises prems33
-                apply(rule conjI)
-                apply(insert prems33(1,2))[1]
-                  apply simp
-                apply(insert prems33(1,3))
-                  apply simp
-                done
-              done
+              apply(rule disjI2)
+                apply simp
+          apply(insert prems25(1,3))
+            apply(erule disjE)
+            apply(rule disjI1)
+              apply simp
             apply(rule disjI2)
               apply(erule conjE)
-              subgoal premises prems34
+              subgoal premises prems26
               apply(rule conjI)
-              apply(insert prems34(1,2))[1]
+              apply(insert prems26(1,2))[1]
+                apply simp
+              apply(insert prems26(1,3))
                 apply(erule conjE)
-                subgoal premises prems35
+                subgoal premises prems27
                 apply(rule conjI)
-                apply(insert prems35(1,2))[1]
-                  apply simp
-                apply(insert prems35(1,3))
-                  apply simp
-                done
-              apply(insert prems34(1,3))
-                apply(erule conjE)
-                subgoal premises prems36
-                apply(rule conjI)
-                apply(insert prems36(1,2))[1]
-                  apply simp
-                apply(insert prems36(1,3))
-                  apply simp
+                apply(insert prems27(1,2))[1]
+                  apply(rule always_imp_refl)
+                apply(insert prems27(1,3))
+                  apply(erule conjE)
+                  subgoal premises prems28
+                  apply(rule conjI)
+                  apply(insert prems28(1,2))[1]
+                    apply(rule always_imp_refl)
+                  apply(insert prems28(1,3))
+                    apply simp
+                  done
                 done
               done
-  done
-apply(insert prems1(1,3,5))
-  apply(erule previous_rule)
-  apply simp
-  apply(rule impI)
-  apply(erule impE)
-  apply assumption
-  subgoal premises prems37
-  apply(insert prems37(1,3))
+          done
+      apply(rule disjI2)
+        apply simp
+    done
+  apply(insert prems21(1,3,5))
+    apply(erule dual_constrained_since_L6)
     apply simp
+    apply(rule impI)
+    apply(erule impE)
+    apply assumption
+    subgoal premises prems29
+    apply(insert prems29(1,3))
+      apply(erule conjE)
+      subgoal premises prems30
+      apply(rule conjI)
+      apply(insert prems30(1,2))[1]
+        apply(erule disjE)
+        apply(rule disjI1)
+          apply simp
+        apply(rule disjI2)
+          apply(erule disjE)
+          apply(rule disjI1)
+            apply simp
+          apply(rule disjI2)
+            apply simp
+      apply(insert prems30(1,3))
+        apply(erule disjE)
+        apply(rule disjI1)
+          apply simp
+        apply(rule disjI2)
+          apply(erule conjE)
+          subgoal premises prems31
+          apply(rule conjI)
+          apply(insert prems31(1,2))[1]
+            apply simp
+          apply(insert prems31(1,3))
+            apply(erule conjE)
+            subgoal premises prems32
+            apply(rule conjI)
+            apply(insert prems32(1,2))[1]
+              apply(rule always_imp_refl)
+            apply(insert prems32(1,3))
+              apply(erule conjE)
+              subgoal premises prems33
+              apply(rule conjI)
+              apply(insert prems33(1,2))[1]
+                apply(rule always_imp_refl)
+              apply(insert prems33(1,3))
+                apply simp
+              done
+            done
+          done
+      done
+    done
   done
 done
 done
 
-lemma EDTL_trigger_prev_final_nontemporal_or_tau_delay_trueeinv_imp_req_gen: "
-EDTL_trigger_prev_final_nontemporal_or_tau_delay_true_inv finalt b_0 t1_0 t1_1_0 t2_1_0 trigger finale release_1 Inv_1 reaction_1 s0 \<Longrightarrow>
+lemma EDTL_final_nontemporal_or_tau_delay_trueeinv_imp_req_gen: "
+EDTL_final_nontemporal_or_tau_delay_true_inv finalt t1_0 b_0 t1_1_0 t2_1_0 trigger finale release_1 Inv_1 reaction_1 s0 \<Longrightarrow>
 toEnvP s0 \<Longrightarrow>
-(True \<and> ((always_imp s0 (\<lambda> r1 . (release_1 s0 r1)) (\<lambda> r1 . (release s0 r1))) \<and> ((((always_imp s0 (\<lambda> r3 . (Inv_1 s0 r3)) (\<lambda> r3 . (Inv s0 r3))) \<and> True) \<and> (((always_imp s0 (\<lambda> r3 . (release_1 s0 r3)) (\<lambda> r3 . (release s0 r3))) \<and> (True \<and> ((always_imp s0 (\<lambda> r3 . (reaction_1 s0 r3)) (\<lambda> r3 . (reaction s0 r3))) \<and> (always_imp s0 (\<lambda> r3 . (Inv_1 s0 r3)) (\<lambda> r3 . (Inv s0 r3)))))) \<and> ((t1_0 s0) <= finalt))) \<and> (((always_imp s0 (\<lambda> r3 . (Inv_1 s0 r3)) (\<lambda> r3 . (Inv s0 r3))) \<and> True) \<and> (((always_imp s0 (\<lambda> r3 . (reaction_1 s0 r3)) (\<lambda> r3 . (reaction s0 r3))) \<and> (always_imp s0 (\<lambda> r3 . (Inv_1 s0 r3)) (\<lambda> r3 . (Inv s0 r3)))) \<and> ((t2_1_0 s0) <= finalt)))))) \<Longrightarrow>
-EDTL_trigger_prev_final_nontemporal_or_tau_delay_true finalt trigger finale release Inv reaction s0"
+((True \<and> ((always_imp s0 (\<lambda> r1 . (release_1 s0 r1)) (\<lambda> r1 . (release s0 r1))) \<and> (((always_imp s0 (\<lambda> r3 . (Inv_1 s0 r3)) (\<lambda> r3 . (Inv s0 r3))) \<and> True) \<and> ((always_imp s0 (\<lambda> r3 . (release_1 s0 r3)) (\<lambda> r3 . (release s0 r3))) \<and> (True \<and> ((always_imp s0 (\<lambda> r3 . (reaction_1 s0 r3)) (\<lambda> r3 . (reaction s0 r3))) \<and> (always_imp s0 (\<lambda> r3 . (Inv_1 s0 r3)) (\<lambda> r3 . (Inv s0 r3))))))))) \<and> ((True \<and> True) \<and> (always_imp s0 (\<lambda> r1 . (reaction_1 s0 r1)) (\<lambda> r1 . (reaction s0 r1))))) \<Longrightarrow>
+EDTL_final_nontemporal_or_tau_delay_true finalt trigger finale release Inv reaction s0"
 
-unfolding EDTL_trigger_prev_final_nontemporal_or_tau_delay_true_inv_def EDTL_trigger_prev_final_nontemporal_or_tau_delay_true_def
-subgoal premises prems1
-apply(insert prems1(1,2))
+unfolding EDTL_final_nontemporal_or_tau_delay_true_inv_def EDTL_final_nontemporal_or_tau_delay_true_def
 apply(erule conjE)
-subgoal premises prems2
-apply(insert prems2(1,2) prems1(3))
-apply(erule always_einv2req)
-apply simp
-  apply(rule always_disj_rule)
+apply(erule conjE)
+subgoal premises prems1
+apply(rule conjI)
+apply(insert prems1(1,2,4))[1]
+  apply(erule always_einv_imp_req_gen)
   apply simp
+    apply(rule always_disj_rule)
+    apply simp
+      apply(erule conjE)
+      subgoal premises prems4
+      apply(rule conjI)
+      apply(insert prems4(1,2))[1]
+        apply(rule always_imp_refl)
+      apply(insert prems4(1,3))
+        apply(rule always_disj_rule)
+        apply simp
+          apply(erule conjE)
+          subgoal premises prems5
+          apply(rule conjI)
+          apply(insert prems5(1,2))[1]
+            apply simp
+          apply(insert prems5(1,3))
+            apply(rule constrained_weak_until_L3)
+            apply simp
+              apply(erule conjE)
+              subgoal premises prems6
+              apply(rule conjI)
+              apply(insert prems6(1,2))[1]
+                apply(rule always_conj_rule)
+                apply simp
+                  apply(erule conjE)
+                  subgoal premises prems7
+                  apply(rule conjI)
+                  apply(insert prems7(1,2))[1]
+                    apply simp
+                  apply(insert prems7(1,3))
+                    apply(rule always_imp_refl)
+                  done
+              apply(insert prems6(1,3))
+                apply(rule always_disj_rule)
+                apply simp
+                  apply(erule conjE)
+                  subgoal premises prems8
+                  apply(rule conjI)
+                  apply(insert prems8(1,2))[1]
+                    apply simp
+                  apply(insert prems8(1,3))
+                    apply(rule always_conj_rule)
+                    apply simp
+                      apply(erule conjE)
+                      subgoal premises prems9
+                      apply(rule conjI)
+                      apply(insert prems9(1,2))[1]
+                        apply(rule always_imp_refl)
+                      apply(insert prems9(1,3))
+                        apply(rule always_conj_rule)
+                        apply simp
+                          apply(erule conjE)
+                          subgoal premises prems10
+                          apply(rule conjI)
+                          apply(insert prems10(1,2))[1]
+                            apply simp
+                          apply(insert prems10(1,3))
+                            apply simp
+                          done
+                      done
+                  done
+              done
+          done
+      done
+apply(insert prems1(1,3,5))
+  subgoal premises prems11
+  apply(insert prems11(1,2))
+  apply(erule conjE)
+  subgoal premises prems12
+  apply(insert prems12(1,2) prems11(3))
+  apply(erule always_einv_imp_req_gen)
+  apply simp
+    apply(rule always_disj_rule)
+    apply simp
+      apply(erule conjE)
+      subgoal premises prems13
+      apply(rule conjI)
+      apply(insert prems13(1,2))[1]
+        apply(rule dual_constrained_since_L5)
+        apply simp
+          apply(erule conjE)
+          subgoal premises prems14
+          apply(rule conjI)
+          apply(insert prems14(1,2))[1]
+            apply(rule always_imp_refl)
+          apply(insert prems14(1,3))
+            apply(rule always_imp_refl)
+          done
+      apply(insert prems13(1,3))
+        apply simp
+      done
+  done
+  done
+done
+done
+
+lemma EDTL_final_nontemporal_or_tau_delay_true_inv_saving: "
+EDTL_final_nontemporal_or_tau_delay_true_inv_part finalt t1_0 b_0 t1_1_0 t2_1_0 trigger finale release Inv reaction s0 \<Longrightarrow>
+consecutive s0 s \<Longrightarrow>
+((((((t1_0 s0) < (finalt + 1)) \<and> ((((release s) \<or> ((finale s) \<and> ((reaction s) \<and> (Inv s)))) \<and> ((t1_0 s) <= ((finalt + 1) + 1))) \<or> (((t1_0 s) <= ((t1_0 s0) + 1)) \<and> ((Inv s) \<and> (\<not> (finale s)))))) \<or> (((t1_0 s0) >= (finalt + 1)) \<and> ((t1_0 s) <= ((t1_0 s0) + 1)))) \<and> ((\<not> (trigger s)) \<or> ((release s) \<or> (((release s) \<or> ((finale s) \<and> ((reaction s) \<and> (Inv s)))) \<or> (((t1_0 s) = 0) \<and> ((Inv s) \<and> (\<not> (finale s)))))))) \<and> (((((finalt > 0) \<or> ((\<not> (trigger s)) \<or> (finale s))) \<and> ((finale s) \<or> ((b_0 s0) \<and> (((t1_1_0 s0) < finalt) \<and> (finalt <= ((t2_1_0 s0) + 1)))))) \<or> (reaction s)) \<and> ((b_0 s) --> ((((t1_1_0 s) > 0) \<or> ((\<not> (trigger s)) \<or> (finale s))) \<and> ((finale s) \<or> ((b_0 s0) \<and> (((t1_1_0 s0) < (t1_1_0 s)) \<and> ((t2_1_0 s) <= ((t2_1_0 s0) + 1))))))))) \<Longrightarrow>
+EDTL_final_nontemporal_or_tau_delay_true_inv_part finalt t1_0 b_0 t1_1_0 t2_1_0 trigger finale release Inv reaction s"
+
+unfolding EDTL_final_nontemporal_or_tau_delay_true_inv_part_def EDTL_final_nontemporal_or_tau_delay_true_part_def
+apply(simp add: EDTL_final_nontemporal_or_tau_delay_true_inv_saving_gen always_imp_refl)
+done
+
+lemma EDTL_final_nontemporal_or_tau_delay_trueeinv_imp_req: "
+EDTL_final_nontemporal_or_tau_delay_true_inv_part finalt t1_0 b_0 t1_1_0 t2_1_0 trigger finale release Inv reaction s \<Longrightarrow>
+toEnvP s \<Longrightarrow>
+True \<Longrightarrow>
+EDTL_final_nontemporal_or_tau_delay_true_part finalt trigger finale release Inv reaction s"
+
+unfolding EDTL_final_nontemporal_or_tau_delay_true_inv_part_def EDTL_final_nontemporal_or_tau_delay_true_part_def
+apply(simp add: EDTL_final_nontemporal_or_tau_delay_trueeinv_imp_req_gen always_imp_refl)
+done
+
+
+
+lemmas EDTL_final_nontemporal_or_tau_delay_true_used_patterns = EDTL_final_nontemporal_or_tau_delay_true_def always_used_patterns constrained_weak_until_def always_used_patterns dual_constrained_since_def 
+
+lemmas EDTL_final_nontemporal_or_tau_delay_true_inv_used_patterns = EDTL_final_nontemporal_or_tau_delay_true_inv_def always_inv_used_patterns constrained_weak_until_inv_def always_inv_used_patterns dual_constrained_since_def dual_constrained_since_inv_def 
+
+lemmas EDTL_final_nontemporal_or_tau_delay_true_inv_part_used_patterns = EDTL_final_nontemporal_or_tau_delay_true_inv_part_def EDTL_final_nontemporal_or_tau_delay_true_inv_used_patterns
+
+lemmas EDTL_final_nontemporal_or_tau_delay_true_part_used_patterns = EDTL_final_nontemporal_or_tau_delay_true_part_def EDTL_final_nontemporal_or_tau_delay_true_used_patterns
+
+definition EDTL_trigger_prev_final_nontemporal_or_tau_delay_true where "EDTL_trigger_prev_final_nontemporal_or_tau_delay_true finalt trigger finale release Inv reaction s \<equiv> ((always (\<lambda> r2 r1 . ((weak_previous (\<lambda> r4 r3 . (\<not> (trigger r3))) r2 r1) \<or> ((release r2 r1) \<or> (constrained_weak_until (finalt + 1) (\<lambda> r4 r3 . ((Inv r4 r3) \<and> (\<not> (finale r3)))) (\<lambda> r4 r3 . ((release r4 r3) \<or> ((finale r3) \<and> ((reaction r4 r3) \<and> (Inv r4 r3))))) r2 r1)))) s) \<and>(always (\<lambda> r2 r1 . ((dual_constrained_since finalt finalt (\<lambda> r4 r3 . (finale r3)) (\<lambda> r4 r3 . ((weak_previous (\<lambda> r6 r5 . (\<not> (trigger r5))) r4 r3) \<or> (finale r3))) r2 r1) \<or> (reaction r2 r1))) s))"
+
+definition EDTL_trigger_prev_final_nontemporal_or_tau_delay_true_part where "EDTL_trigger_prev_final_nontemporal_or_tau_delay_true_part finalt trigger finale release Inv reaction s \<equiv> (EDTL_trigger_prev_final_nontemporal_or_tau_delay_true finalt trigger finale (\<lambda> s s1 . (release s1)) (\<lambda> s s1 . (Inv s1)) (\<lambda> s s1 . (reaction s1)) s)"
+
+definition EDTL_trigger_prev_final_nontemporal_or_tau_delay_true_inv where "EDTL_trigger_prev_final_nontemporal_or_tau_delay_true_inv finalt b_0 t1_0 b_1 b_2 t1_1_0 t2_1_0 trigger finale release_1 Inv_1 reaction_1 s \<equiv> (((always_inv (\<lambda> r2 r1 . ((weak_previous (\<lambda> r4 r3 . (\<not> (trigger r3))) r2 r1) \<or> ((release_1 r2 r1) \<or> (constrained_weak_until_inv (finalt + 1) t1_0 (\<lambda> r4 r3 . ((Inv_1 r4 r3) \<and> (\<not> (finale r3)))) (\<lambda> r4 r3 . ((release_1 r4 r3) \<or> ((finale r3) \<and> ((reaction_1 r4 r3) \<and> (Inv_1 r4 r3))))) r2 r1)))) s) \<and> (previous_inv b_0 (\<lambda> r4 r3 . (\<not> (trigger r3))) s)) \<and> (((always_inv (\<lambda> r2 r1 . ((dual_constrained_since finalt finalt (\<lambda> r4 r3 . (finale r3)) (\<lambda> r4 r3 . ((weak_previous (\<lambda> r6 r5 . (\<not> (trigger r5))) r4 r3) \<or> (finale r3))) r2 r1) \<or> (reaction_1 r2 r1))) s) \<and> (dual_constrained_since_inv finalt finalt b_2 t1_1_0 t2_1_0 (\<lambda> r4 r3 . (finale r3)) (\<lambda> r4 r3 . ((weak_previous (\<lambda> r6 r5 . (\<not> (trigger r5))) r4 r3) \<or> (finale r3))) s)) \<and> (previous_inv b_1 (\<lambda> r6 r5 . (\<not> (trigger r5))) s)))"
+
+definition EDTL_trigger_prev_final_nontemporal_or_tau_delay_true_inv_part where "EDTL_trigger_prev_final_nontemporal_or_tau_delay_true_inv_part finalt b_0 t1_0 b_1 b_2 t1_1_0 t2_1_0 trigger finale release Inv reaction s \<equiv> (EDTL_trigger_prev_final_nontemporal_or_tau_delay_true_inv finalt b_0 t1_0 b_1 b_2 t1_1_0 t2_1_0 trigger finale (\<lambda> s s1 . (release s1)) (\<lambda> s s1 . (Inv s1)) (\<lambda> s s1 . (reaction s1)) s)"
+
+lemma EDTL_trigger_prev_final_nontemporal_or_tau_delay_true_inv_saving_gen: "
+EDTL_trigger_prev_final_nontemporal_or_tau_delay_true_inv finalt b_0 t1_0 b_1 b_2 t1_1_0 t2_1_0 trigger finale release_1 Inv_1 reaction_1 s0 \<Longrightarrow>
+consecutive s0 s \<Longrightarrow>
+((((True \<and> ((always_imp s0 (\<lambda> r1 . (release_1 s0 r1)) (\<lambda> r1 . (release_1 s r1))) \<and> (((always_imp s0 (\<lambda> r3 . (Inv_1 s0 r3)) (\<lambda> r3 . (Inv_1 s r3))) \<and> True) \<and> (((always_imp s0 (\<lambda> r3 . (release_1 s0 r3)) (\<lambda> r3 . (release_1 s r3))) \<and> (True \<and> ((always_imp s0 (\<lambda> r3 . (reaction_1 s0 r3)) (\<lambda> r3 . (reaction_1 s r3))) \<and> (always_imp s0 (\<lambda> r3 . (Inv_1 s0 r3)) (\<lambda> r3 . (Inv_1 s r3)))))) \<and> ((((t1_0 s0) < (finalt + 1)) \<and> ((((release_1 s s) \<or> ((finale s) \<and> ((reaction_1 s s) \<and> (Inv_1 s s)))) \<and> ((t1_0 s) <= ((finalt + 1) + 1))) \<or> (((t1_0 s) <= ((t1_0 s0) + 1)) \<and> ((Inv_1 s s) \<and> (\<not> (finale s)))))) \<or> (((t1_0 s0) >= (finalt + 1)) \<and> ((t1_0 s) <= ((t1_0 s0) + 1)))))))) \<and> (((b_0 s0) \<and> True) \<or> ((release_1 s s) \<or> (((release_1 s s) \<or> ((finale s) \<and> ((reaction_1 s s) \<and> (Inv_1 s s)))) \<or> (((t1_0 s) = 0) \<and> ((Inv_1 s s) \<and> (\<not> (finale s)))))))) \<and> ((b_0 s) --> (\<not> (trigger s)))) \<and> (((((True \<and> (True \<and> True)) \<and> (always_imp s0 (\<lambda> r1 . (reaction_1 s0 r1)) (\<lambda> r1 . (reaction_1 s r1)))) \<and> ((((finalt > 0) \<or> (((b_1 s0) \<and> True) \<or> (finale s))) \<and> ((finale s) \<or> ((b_2 s0) \<and> (True \<and> ((True \<and> True) \<and> (((t1_1_0 s0) < finalt) \<and> (finalt <= ((t2_1_0 s0) + 1)))))))) \<or> (reaction_1 s s))) \<and> ((b_2 s) --> ((((t1_1_0 s) > 0) \<or> (((b_1 s0) \<and> True) \<or> (finale s))) \<and> ((finale s) \<or> ((b_2 s0) \<and> (True \<and> ((True \<and> True) \<and> (((t1_1_0 s0) < (t1_1_0 s)) \<and> ((t2_1_0 s) <= ((t2_1_0 s0) + 1)))))))))) \<and> ((b_1 s) --> (\<not> (trigger s))))) \<Longrightarrow>
+EDTL_trigger_prev_final_nontemporal_or_tau_delay_true_inv finalt b_0 t1_0 b_1 b_2 t1_1_0 t2_1_0 trigger finale release_1 Inv_1 reaction_1 s"
+
+unfolding EDTL_trigger_prev_final_nontemporal_or_tau_delay_true_inv_def
+apply(erule conjE)
+apply(erule conjE)
+subgoal premises prems1
+apply(rule conjI)
+apply(insert prems1(1,2,4))[1]
+  apply(erule conjE)
+  apply(erule conjE)
+  subgoal premises prems2
+  apply(rule conjI)
+  apply(insert prems2(1,2,4))[1]
+  apply(erule always_inv_saving_gen)
+    apply simp
     apply(erule conjE)
     subgoal premises prems3
     apply(rule conjI)
     apply(insert prems3(1,2))[1]
-      apply(rule weak_previous_LS5)
-      apply simp
-        apply(rule always_imp_refl)
-    apply(insert prems3(1,3))
       apply(rule always_disj_rule)
       apply simp
         apply(erule conjE)
         subgoal premises prems4
         apply(rule conjI)
         apply(insert prems4(1,2))[1]
+          apply(rule weak_previous_L4)
           apply simp
+            apply(rule always_imp_refl)
         apply(insert prems4(1,3))
           apply(rule always_disj_rule)
           apply simp
@@ -2270,7 +1907,9 @@ apply simp
             subgoal premises prems5
             apply(rule conjI)
             apply(insert prems5(1,2))[1]
-              apply(rule constrained_until_einv2req)
+              apply simp
+            apply(insert prems5(1,3))
+              apply(rule constrained_weak_until_L1)
               apply simp
                 apply(erule conjE)
                 subgoal premises prems6
@@ -2320,66 +1959,480 @@ apply simp
                           done
                       done
                   apply(insert prems8(1,3))
-                    apply simp
-                  done
-                done
-            apply(insert prems5(1,3))
-              apply(rule constrained_until2_einv2req)
-              apply simp
-                apply(erule conjE)
-                subgoal premises prems12
-                apply(rule conjI)
-                apply(insert prems12(1,2))[1]
-                  apply(rule always_conj_rule)
-                  apply simp
-                    apply(erule conjE)
-                    subgoal premises prems13
-                    apply(rule conjI)
-                    apply(insert prems13(1,2))[1]
-                      apply simp
-                    apply(insert prems13(1,3))
-                      apply(rule always_imp_refl)
-                    done
-                apply(insert prems12(1,3))
-                  apply(erule conjE)
-                  subgoal premises prems14
-                  apply(rule conjI)
-                  apply(insert prems14(1,2))[1]
-                    apply(rule always_conj_rule)
-                    apply simp
+                    apply(erule disjE)
+                    apply(rule disjI1)
                       apply(erule conjE)
-                      subgoal premises prems15
+                      subgoal premises prems12
                       apply(rule conjI)
-                      apply(insert prems15(1,2))[1]
+                      apply(insert prems12(1,2))[1]
                         apply simp
-                      apply(insert prems15(1,3))
-                        apply simp
+                      apply(insert prems12(1,3))
+                        apply(erule disjE)
+                        apply(rule disjI1)
+                          apply(erule conjE)
+                          subgoal premises prems13
+                          apply(rule conjI)
+                          apply(insert prems13(1,2))[1]
+                            apply(erule disjE)
+                            apply(rule disjI1)
+                              apply simp
+                            apply(rule disjI2)
+                              apply(erule conjE)
+                              subgoal premises prems14
+                              apply(rule conjI)
+                              apply(insert prems14(1,2))[1]
+                                apply simp
+                              apply(insert prems14(1,3))
+                                apply(erule conjE)
+                                subgoal premises prems15
+                                apply(rule conjI)
+                                apply(insert prems15(1,2))[1]
+                                  apply simp
+                                apply(insert prems15(1,3))
+                                  apply simp
+                                done
+                              done
+                          apply(insert prems13(1,3))
+                            apply simp
+                          done
+                        apply(rule disjI2)
+                          apply(erule conjE)
+                          subgoal premises prems16
+                          apply(rule conjI)
+                          apply(insert prems16(1,2))[1]
+                            apply simp
+                          apply(insert prems16(1,3))
+                            apply(erule conjE)
+                            subgoal premises prems17
+                            apply(rule conjI)
+                            apply(insert prems17(1,2))[1]
+                              apply simp
+                            apply(insert prems17(1,3))
+                              apply simp
+                            done
+                          done
                       done
-                  apply(insert prems14(1,3))
-                    apply simp
+                    apply(rule disjI2)
+                      apply simp
                   done
                 done
             done
         done
+    apply(insert prems3(1,3))
+      apply(erule disjE)
+      apply(rule disjI1)
+        apply(rule weak_previous_L7[OF prems2(3)])
+        apply simp
+          apply(erule conjE)
+          subgoal premises prems18
+          apply(rule conjI)
+          apply(insert prems18(1,2))[1]
+            apply simp
+          apply(insert prems18(1,3))
+            apply(rule always_imp_refl)
+          done
+      apply(rule disjI2)
+        apply(erule disjE)
+        apply(rule disjI1)
+          apply simp
+        apply(rule disjI2)
+          apply(rule constrained_weak_until_L2)
+          apply simp
+            apply(erule disjE)
+            apply(rule disjI1)
+              apply(erule disjE)
+              apply(rule disjI1)
+                apply simp
+              apply(rule disjI2)
+                apply(erule conjE)
+                subgoal premises prems19
+                apply(rule conjI)
+                apply(insert prems19(1,2))[1]
+                  apply simp
+                apply(insert prems19(1,3))
+                  apply(erule conjE)
+                  subgoal premises prems20
+                  apply(rule conjI)
+                  apply(insert prems20(1,2))[1]
+                    apply simp
+                  apply(insert prems20(1,3))
+                    apply simp
+                  done
+                done
+            apply(rule disjI2)
+              apply(erule conjE)
+              subgoal premises prems21
+              apply(rule conjI)
+              apply(insert prems21(1,2))[1]
+                apply simp
+              apply(insert prems21(1,3))
+                apply(erule conjE)
+                subgoal premises prems22
+                apply(rule conjI)
+                apply(insert prems22(1,2))[1]
+                  apply simp
+                apply(insert prems22(1,3))
+                  apply simp
+                done
+              done
     done
+  apply(insert prems2(1,3,5))
+    apply(erule previous_inv_L6)
+    apply simp
+    apply(rule impI)
+    apply(erule impE)
+    apply assumption
+    subgoal premises prems23
+    apply(insert prems23(1,3))
+      apply simp
+    done
+  done
+apply(insert prems1(1,3,5))
+  apply(erule conjE)
+  apply(erule conjE)
+  subgoal premises prems24
+  apply(rule conjI)
+  apply(insert prems24(1,2,4))[1]
+  apply(erule conjE)
+  apply(erule conjE)
+  subgoal premises prems25
+  apply(rule conjI)
+  apply(insert prems25(1,2,4))[1]
+  apply(erule always_inv_saving_gen)
+    apply simp
+    apply(erule conjE)
+    subgoal premises prems26
+    apply(rule conjI)
+    apply(insert prems26(1,2))[1]
+      apply(rule always_disj_rule)
+      apply simp
+        apply(erule conjE)
+        subgoal premises prems27
+        apply(rule conjI)
+        apply(insert prems27(1,2))[1]
+          apply(rule dual_constrained_since_L4)
+          apply simp
+            apply(erule conjE)
+            subgoal premises prems28
+            apply(rule conjI)
+            apply(insert prems28(1,2))[1]
+              apply(rule always_imp_refl)
+            apply(insert prems28(1,3))
+              apply(rule always_disj_rule)
+              apply simp
+                apply(erule conjE)
+                subgoal premises prems29
+                apply(rule conjI)
+                apply(insert prems29(1,2))[1]
+                  apply(rule weak_previous_L4)
+                  apply simp
+                    apply(rule always_imp_refl)
+                apply(insert prems29(1,3))
+                  apply(rule always_imp_refl)
+                done
+            done
+        apply(insert prems27(1,3))
+          apply simp
+        done
+    apply(insert prems26(1,3))
+      apply(erule disjE)
+      apply(rule disjI1)
+        apply(rule dual_constrained_since_L7[OF prems25(3)])
+        apply simp
+          apply(erule conjE)
+          subgoal premises prems30
+          apply(rule conjI)
+          apply(insert prems30(1,2))[1]
+            apply(erule disjE)
+            apply(rule disjI1)
+              apply simp
+            apply(rule disjI2)
+              apply(erule disjE)
+              apply(rule disjI1)
+                apply(rule weak_previous_L7[OF prems24(3)])
+                apply simp
+                  apply(erule conjE)
+                  subgoal premises prems31
+                  apply(rule conjI)
+                  apply(insert prems31(1,2))[1]
+                    apply simp
+                  apply(insert prems31(1,3))
+                    apply(rule always_imp_refl)
+                  done
+              apply(rule disjI2)
+                apply simp
+          apply(insert prems30(1,3))
+            apply(erule disjE)
+            apply(rule disjI1)
+              apply simp
+            apply(rule disjI2)
+              apply(erule conjE)
+              subgoal premises prems32
+              apply(rule conjI)
+              apply(insert prems32(1,2))[1]
+                apply simp
+              apply(insert prems32(1,3))
+                apply(erule conjE)
+                subgoal premises prems33
+                apply(rule conjI)
+                apply(insert prems33(1,2))[1]
+                  apply(rule always_imp_refl)
+                apply(insert prems33(1,3))
+                  apply(erule conjE)
+                  subgoal premises prems34
+                  apply(rule conjI)
+                  apply(insert prems34(1,2))[1]
+                    apply(rule always_disj_rule)
+                    apply simp
+                      apply(erule conjE)
+                      subgoal premises prems35
+                      apply(rule conjI)
+                      apply(insert prems35(1,2))[1]
+                        apply(rule weak_previous_L4)
+                        apply simp
+                          apply(rule always_imp_refl)
+                      apply(insert prems35(1,3))
+                        apply(rule always_imp_refl)
+                      done
+                  apply(insert prems34(1,3))
+                    apply simp
+                  done
+                done
+              done
+          done
+      apply(rule disjI2)
+        apply simp
+    done
+  apply(insert prems25(1,3,5))
+    apply(erule dual_constrained_since_L6)
+    apply simp
+    apply(rule impI)
+    apply(erule impE)
+    apply assumption
+    subgoal premises prems36
+    apply(insert prems36(1,3))
+      apply(erule conjE)
+      subgoal premises prems37
+      apply(rule conjI)
+      apply(insert prems37(1,2))[1]
+        apply(erule disjE)
+        apply(rule disjI1)
+          apply simp
+        apply(rule disjI2)
+          apply(erule disjE)
+          apply(rule disjI1)
+            apply(rule weak_previous_L7[OF prems24(3)])
+            apply simp
+              apply(erule conjE)
+              subgoal premises prems38
+              apply(rule conjI)
+              apply(insert prems38(1,2))[1]
+                apply simp
+              apply(insert prems38(1,3))
+                apply(rule always_imp_refl)
+              done
+          apply(rule disjI2)
+            apply simp
+      apply(insert prems37(1,3))
+        apply(erule disjE)
+        apply(rule disjI1)
+          apply simp
+        apply(rule disjI2)
+          apply(erule conjE)
+          subgoal premises prems39
+          apply(rule conjI)
+          apply(insert prems39(1,2))[1]
+            apply simp
+          apply(insert prems39(1,3))
+            apply(erule conjE)
+            subgoal premises prems40
+            apply(rule conjI)
+            apply(insert prems40(1,2))[1]
+              apply(rule always_imp_refl)
+            apply(insert prems40(1,3))
+              apply(erule conjE)
+              subgoal premises prems41
+              apply(rule conjI)
+              apply(insert prems41(1,2))[1]
+                apply(rule always_disj_rule)
+                apply simp
+                  apply(erule conjE)
+                  subgoal premises prems42
+                  apply(rule conjI)
+                  apply(insert prems42(1,2))[1]
+                    apply(rule weak_previous_L4)
+                    apply simp
+                      apply(rule always_imp_refl)
+                  apply(insert prems42(1,3))
+                    apply(rule always_imp_refl)
+                  done
+              apply(insert prems41(1,3))
+                apply simp
+              done
+            done
+          done
+      done
+    done
+  done
+  apply(insert prems24(1,3,5))
+    apply(erule previous_inv_L6)
+    apply simp
+    apply(rule impI)
+    apply(erule impE)
+    apply assumption
+    subgoal premises prems43
+    apply(insert prems43(1,3))
+      apply simp
+    done
+  done
 done
+done
+
+lemma EDTL_trigger_prev_final_nontemporal_or_tau_delay_trueeinv_imp_req_gen: "
+EDTL_trigger_prev_final_nontemporal_or_tau_delay_true_inv finalt b_0 t1_0 b_1 b_2 t1_1_0 t2_1_0 trigger finale release_1 Inv_1 reaction_1 s0 \<Longrightarrow>
+toEnvP s0 \<Longrightarrow>
+((True \<and> ((always_imp s0 (\<lambda> r1 . (release_1 s0 r1)) (\<lambda> r1 . (release s0 r1))) \<and> (((always_imp s0 (\<lambda> r3 . (Inv_1 s0 r3)) (\<lambda> r3 . (Inv s0 r3))) \<and> True) \<and> ((always_imp s0 (\<lambda> r3 . (release_1 s0 r3)) (\<lambda> r3 . (release s0 r3))) \<and> (True \<and> ((always_imp s0 (\<lambda> r3 . (reaction_1 s0 r3)) (\<lambda> r3 . (reaction s0 r3))) \<and> (always_imp s0 (\<lambda> r3 . (Inv_1 s0 r3)) (\<lambda> r3 . (Inv s0 r3))))))))) \<and> ((True \<and> (True \<and> True)) \<and> (always_imp s0 (\<lambda> r1 . (reaction_1 s0 r1)) (\<lambda> r1 . (reaction s0 r1))))) \<Longrightarrow>
+EDTL_trigger_prev_final_nontemporal_or_tau_delay_true finalt trigger finale release Inv reaction s0"
+
+unfolding EDTL_trigger_prev_final_nontemporal_or_tau_delay_true_inv_def EDTL_trigger_prev_final_nontemporal_or_tau_delay_true_def
+apply(erule conjE)
+apply(erule conjE)
+subgoal premises prems1
+apply(rule conjI)
+apply(insert prems1(1,2,4))[1]
+  subgoal premises prems2
+  apply(insert prems2(1,2))
+  apply(erule conjE)
+  subgoal premises prems3
+  apply(insert prems3(1,2) prems2(3))
+  apply(erule always_einv_imp_req_gen)
+  apply simp
+    apply(rule always_disj_rule)
+    apply simp
+      apply(erule conjE)
+      subgoal premises prems4
+      apply(rule conjI)
+      apply(insert prems4(1,2))[1]
+        apply(rule weak_previous_L5)
+        apply simp
+          apply(rule always_imp_refl)
+      apply(insert prems4(1,3))
+        apply(rule always_disj_rule)
+        apply simp
+          apply(erule conjE)
+          subgoal premises prems5
+          apply(rule conjI)
+          apply(insert prems5(1,2))[1]
+            apply simp
+          apply(insert prems5(1,3))
+            apply(rule constrained_weak_until_L3)
+            apply simp
+              apply(erule conjE)
+              subgoal premises prems6
+              apply(rule conjI)
+              apply(insert prems6(1,2))[1]
+                apply(rule always_conj_rule)
+                apply simp
+                  apply(erule conjE)
+                  subgoal premises prems7
+                  apply(rule conjI)
+                  apply(insert prems7(1,2))[1]
+                    apply simp
+                  apply(insert prems7(1,3))
+                    apply(rule always_imp_refl)
+                  done
+              apply(insert prems6(1,3))
+                apply(rule always_disj_rule)
+                apply simp
+                  apply(erule conjE)
+                  subgoal premises prems8
+                  apply(rule conjI)
+                  apply(insert prems8(1,2))[1]
+                    apply simp
+                  apply(insert prems8(1,3))
+                    apply(rule always_conj_rule)
+                    apply simp
+                      apply(erule conjE)
+                      subgoal premises prems9
+                      apply(rule conjI)
+                      apply(insert prems9(1,2))[1]
+                        apply(rule always_imp_refl)
+                      apply(insert prems9(1,3))
+                        apply(rule always_conj_rule)
+                        apply simp
+                          apply(erule conjE)
+                          subgoal premises prems10
+                          apply(rule conjI)
+                          apply(insert prems10(1,2))[1]
+                            apply simp
+                          apply(insert prems10(1,3))
+                            apply simp
+                          done
+                      done
+                  done
+              done
+          done
+      done
+  done
+  done
+apply(insert prems1(1,3,5))
+  subgoal premises prems11
+  apply(insert prems11(1,2))
+  apply(simp only: conj_assoc)
+  apply(erule conjE)
+  subgoal premises prems12
+  apply(insert prems12(1,2) prems11(3))
+  apply(erule always_einv_imp_req_gen)
+  apply simp
+    apply(rule always_disj_rule)
+    apply simp
+      apply(erule conjE)
+      subgoal premises prems13
+      apply(rule conjI)
+      apply(insert prems13(1,2))[1]
+        apply(rule dual_constrained_since_L5)
+        apply simp
+          apply(erule conjE)
+          subgoal premises prems14
+          apply(rule conjI)
+          apply(insert prems14(1,2))[1]
+            apply(rule always_imp_refl)
+          apply(insert prems14(1,3))
+            apply(rule always_disj_rule)
+            apply simp
+              apply(erule conjE)
+              subgoal premises prems15
+              apply(rule conjI)
+              apply(insert prems15(1,2))[1]
+                apply(rule weak_previous_L5)
+                apply simp
+                  apply(rule always_imp_refl)
+              apply(insert prems15(1,3))
+                apply(rule always_imp_refl)
+              done
+          done
+      apply(insert prems13(1,3))
+        apply simp
+      done
+  done
+  done
 done
 done
 
 lemma EDTL_trigger_prev_final_nontemporal_or_tau_delay_true_inv_saving: "
-EDTL_trigger_prev_final_nontemporal_or_tau_delay_true_inv_part finalt b_0 t1_0 t1_1_0 t2_1_0 trigger finale release Inv reaction s0 \<Longrightarrow>
+EDTL_trigger_prev_final_nontemporal_or_tau_delay_true_inv_part finalt b_0 t1_0 b_1 b_2 t1_1_0 t2_1_0 trigger finale release Inv reaction s0 \<Longrightarrow>
 consecutive s0 s \<Longrightarrow>
-((((((t1_0 s0) = 0) \<or> ((((release s) \<or> ((finale s) \<and> ((reaction s) \<and> (Inv s)))) \<and> ((t1_0 s0) <= finalt)) \<or> (((Inv s) \<and> (\<not> (finale s))) \<and> ((t1_0 s0) < (t1_0 s))))) \<and> (((t2_1_0 s0) = 0) \<or> (((t1_1_0 s0) >= (t2_1_0 s0)) \<or> ((((reaction s) \<and> (Inv s)) \<and> ((((t1_1_0 s0) + 1) >= finalt) \<and> ((t2_1_0 s0) <= finalt))) \<or> (((Inv s) \<and> (\<not> (finale s))) \<and> ((((t1_1_0 s0) + 1) >= (t1_1_0 s)) \<and> ((t2_1_0 s0) < (t2_1_0 s)))))))) \<and> ((b_0 s0) \<or> ((release s) \<or> ((((release s) \<or> ((finale s) \<and> ((reaction s) \<and> (Inv s)))) \<or> (((Inv s) \<and> (\<not> (finale s))) \<and> ((t1_0 s) > 0))) \<or> (((finalt = 0) \<and> ((reaction s) \<and> (Inv s))) \<or> (((Inv s) \<and> (\<not> (finale s))) \<and> (((t1_1_0 s) = 0) \<and> ((t2_1_0 s) > 0)))))))) \<and> ((b_0 s) --> (\<not> (trigger s)))) \<Longrightarrow>
-EDTL_trigger_prev_final_nontemporal_or_tau_delay_true_inv_part finalt b_0 t1_0 t1_1_0 t2_1_0 trigger finale release Inv reaction s"
+(((((((t1_0 s0) < (finalt + 1)) \<and> ((((release s) \<or> ((finale s) \<and> ((reaction s) \<and> (Inv s)))) \<and> ((t1_0 s) <= ((finalt + 1) + 1))) \<or> (((t1_0 s) <= ((t1_0 s0) + 1)) \<and> ((Inv s) \<and> (\<not> (finale s)))))) \<or> (((t1_0 s0) >= (finalt + 1)) \<and> ((t1_0 s) <= ((t1_0 s0) + 1)))) \<and> ((b_0 s0) \<or> ((release s) \<or> (((release s) \<or> ((finale s) \<and> ((reaction s) \<and> (Inv s)))) \<or> (((t1_0 s) = 0) \<and> ((Inv s) \<and> (\<not> (finale s)))))))) \<and> ((b_0 s) --> (\<not> (trigger s)))) \<and> ((((((finalt > 0) \<or> ((b_1 s0) \<or> (finale s))) \<and> ((finale s) \<or> ((b_2 s0) \<and> (((t1_1_0 s0) < finalt) \<and> (finalt <= ((t2_1_0 s0) + 1)))))) \<or> (reaction s)) \<and> ((b_2 s) --> ((((t1_1_0 s) > 0) \<or> ((b_1 s0) \<or> (finale s))) \<and> ((finale s) \<or> ((b_2 s0) \<and> (((t1_1_0 s0) < (t1_1_0 s)) \<and> ((t2_1_0 s) <= ((t2_1_0 s0) + 1)))))))) \<and> ((b_1 s) --> (\<not> (trigger s))))) \<Longrightarrow>
+EDTL_trigger_prev_final_nontemporal_or_tau_delay_true_inv_part finalt b_0 t1_0 b_1 b_2 t1_1_0 t2_1_0 trigger finale release Inv reaction s"
 
 unfolding EDTL_trigger_prev_final_nontemporal_or_tau_delay_true_inv_part_def EDTL_trigger_prev_final_nontemporal_or_tau_delay_true_part_def
 apply(simp add: EDTL_trigger_prev_final_nontemporal_or_tau_delay_true_inv_saving_gen always_imp_refl)
 done
 
 lemma EDTL_trigger_prev_final_nontemporal_or_tau_delay_trueeinv_imp_req: "
-EDTL_trigger_prev_final_nontemporal_or_tau_delay_true_inv_part finalt b_0 t1_0 t1_1_0 t2_1_0 trigger finale release Inv reaction s \<Longrightarrow>
+EDTL_trigger_prev_final_nontemporal_or_tau_delay_true_inv_part finalt b_0 t1_0 b_1 b_2 t1_1_0 t2_1_0 trigger finale release Inv reaction s \<Longrightarrow>
 toEnvP s \<Longrightarrow>
-(((t1_0 s) <= finalt) \<and> ((t2_1_0 s) <= finalt)) \<Longrightarrow>
+True \<Longrightarrow>
 EDTL_trigger_prev_final_nontemporal_or_tau_delay_true_part finalt trigger finale release Inv reaction s"
 
 unfolding EDTL_trigger_prev_final_nontemporal_or_tau_delay_true_inv_part_def EDTL_trigger_prev_final_nontemporal_or_tau_delay_true_part_def
@@ -2388,19 +2441,19 @@ done
 
 
 
-lemmas EDTL_trigger_prev_final_nontemporal_or_tau_delay_true_used_patterns = EDTL_trigger_prev_final_nontemporal_or_tau_delay_true_def always_used_patterns weak_previous_def constrained_until_def constrained_until2_def 
+lemmas EDTL_trigger_prev_final_nontemporal_or_tau_delay_true_used_patterns = EDTL_trigger_prev_final_nontemporal_or_tau_delay_true_def always_used_patterns weak_previous_def constrained_weak_until_def always_used_patterns dual_constrained_since_def weak_previous_def 
 
-lemmas EDTL_trigger_prev_final_nontemporal_or_tau_delay_true_inv_used_patterns = EDTL_trigger_prev_final_nontemporal_or_tau_delay_true_inv_def always_inv_used_patterns weak_previous_def constrained_until_inv_def constrained_until2_inv_def previous_inv_def 
+lemmas EDTL_trigger_prev_final_nontemporal_or_tau_delay_true_inv_used_patterns = EDTL_trigger_prev_final_nontemporal_or_tau_delay_true_inv_def always_inv_used_patterns weak_previous_def constrained_weak_until_inv_def previous_inv_def always_inv_used_patterns dual_constrained_since_def weak_previous_def dual_constrained_since_inv_def weak_previous_def previous_inv_def 
 
 lemmas EDTL_trigger_prev_final_nontemporal_or_tau_delay_true_inv_part_used_patterns = EDTL_trigger_prev_final_nontemporal_or_tau_delay_true_inv_part_def EDTL_trigger_prev_final_nontemporal_or_tau_delay_true_inv_used_patterns
 
 lemmas EDTL_trigger_prev_final_nontemporal_or_tau_delay_true_part_used_patterns = EDTL_trigger_prev_final_nontemporal_or_tau_delay_true_part_def EDTL_trigger_prev_final_nontemporal_or_tau_delay_true_used_patterns
 
-definition EDTL_release_false_final_tau_delay_tau where "EDTL_release_false_final_tau_delay_tau fin delay trigger Inv reaction s \<equiv> (always (\<lambda> r2 r1 . ((\<not> (trigger r1)) \<or> (constrained_until2 fin (fin + delay) Inv (\<lambda> r4 r3 . ((reaction r4 r3) \<and> (Inv r4 r3))) r2 r1))) s)"
+definition EDTL_release_false_final_tau_delay_tau where "EDTL_release_false_final_tau_delay_tau fin delay trigger Inv reaction s \<equiv> (always (\<lambda> r2 r1 . ((\<not> (trigger r1)) \<or> (constrained_until fin (fin + delay) Inv (\<lambda> r4 r3 . ((reaction r4 r3) \<and> (Inv r4 r3))) r2 r1))) s)"
 
 definition EDTL_release_false_final_tau_delay_tau_part where "EDTL_release_false_final_tau_delay_tau_part fin delay trigger Inv reaction s \<equiv> (EDTL_release_false_final_tau_delay_tau fin delay trigger (\<lambda> s s1 . (Inv s1)) (\<lambda> s s1 . (reaction s1)) s)"
 
-definition EDTL_release_false_final_tau_delay_tau_inv where "EDTL_release_false_final_tau_delay_tau_inv fin delay t1_1_0 t2_1_0 trigger Inv_1 reaction_1 s \<equiv> (always_inv (\<lambda> r2 r1 . ((\<not> (trigger r1)) \<or> (constrained_until2_inv fin (fin + delay) t1_1_0 t2_1_0 Inv_1 (\<lambda> r4 r3 . ((reaction_1 r4 r3) \<and> (Inv_1 r4 r3))) r2 r1))) s)"
+definition EDTL_release_false_final_tau_delay_tau_inv where "EDTL_release_false_final_tau_delay_tau_inv fin delay t1_1_0 t2_1_0 trigger Inv_1 reaction_1 s \<equiv> (always_inv (\<lambda> r2 r1 . ((\<not> (trigger r1)) \<or> (constrained_until_inv fin (fin + delay) t1_1_0 t2_1_0 Inv_1 (\<lambda> r4 r3 . ((reaction_1 r4 r3) \<and> (Inv_1 r4 r3))) r2 r1))) s)"
 
 definition EDTL_release_false_final_tau_delay_tau_inv_part where "EDTL_release_false_final_tau_delay_tau_inv_part fin delay t1_1_0 t2_1_0 trigger Inv reaction s \<equiv> (EDTL_release_false_final_tau_delay_tau_inv fin delay t1_1_0 t2_1_0 trigger (\<lambda> s s1 . (Inv s1)) (\<lambda> s s1 . (reaction s1)) s)"
 
@@ -2411,7 +2464,7 @@ consecutive s0 s \<Longrightarrow>
 EDTL_release_false_final_tau_delay_tau_inv fin delay t1_1_0 t2_1_0 trigger Inv_1 reaction_1 s"
 
 unfolding EDTL_release_false_final_tau_delay_tau_inv_def
-apply(erule always_rule)
+apply(erule always_inv_saving_gen)
   apply simp
   apply(erule conjE)
   subgoal premises prems1
@@ -2425,7 +2478,7 @@ apply(erule always_rule)
       apply(insert prems2(1,2))[1]
         apply(rule always_imp_refl)
       apply(insert prems2(1,3))
-        apply(rule constrained_until2_rule)
+        apply(rule constrained_until_L1)
         apply simp
           apply(erule conjE)
           subgoal premises prems3
@@ -2504,7 +2557,7 @@ apply(erule always_rule)
     apply(rule disjI1)
       apply simp
     apply(rule disjI2)
-      apply(rule constrained_until2_one_point)
+      apply(rule constrained_until_L2)
       apply simp
         apply(erule disjE)
         apply(rule disjI1)
@@ -2549,7 +2602,7 @@ toEnvP s0 \<Longrightarrow>
 EDTL_release_false_final_tau_delay_tau fin delay trigger Inv reaction s0"
 
 unfolding EDTL_release_false_final_tau_delay_tau_inv_def EDTL_release_false_final_tau_delay_tau_def
-apply(erule always_einv2req)
+apply(erule always_einv_imp_req_gen)
 apply simp
   apply(rule always_disj_rule)
   apply simp
@@ -2559,7 +2612,7 @@ apply simp
     apply(insert prems3(1,2))[1]
       apply(rule always_imp_refl)
     apply(insert prems3(1,3))
-      apply(rule constrained_until2_einv2req)
+      apply(rule constrained_until_L3)
       apply simp
         apply(erule conjE)
         subgoal premises prems4
@@ -2610,19 +2663,19 @@ done
 
 
 
-lemmas EDTL_release_false_final_tau_delay_tau_used_patterns = EDTL_release_false_final_tau_delay_tau_def always_used_patterns constrained_until2_def 
+lemmas EDTL_release_false_final_tau_delay_tau_used_patterns = EDTL_release_false_final_tau_delay_tau_def always_used_patterns constrained_until_def 
 
-lemmas EDTL_release_false_final_tau_delay_tau_inv_used_patterns = EDTL_release_false_final_tau_delay_tau_inv_def always_inv_used_patterns constrained_until2_inv_def 
+lemmas EDTL_release_false_final_tau_delay_tau_inv_used_patterns = EDTL_release_false_final_tau_delay_tau_inv_def always_inv_used_patterns constrained_until_inv_def 
 
 lemmas EDTL_release_false_final_tau_delay_tau_inv_part_used_patterns = EDTL_release_false_final_tau_delay_tau_inv_part_def EDTL_release_false_final_tau_delay_tau_inv_used_patterns
 
 lemmas EDTL_release_false_final_tau_delay_tau_part_used_patterns = EDTL_release_false_final_tau_delay_tau_part_def EDTL_release_false_final_tau_delay_tau_used_patterns
 
-definition EDTL_trigger_prev_release_false_final_tau_delay_tau where "EDTL_trigger_prev_release_false_final_tau_delay_tau fin delay trigger Inv reaction s \<equiv> (always (\<lambda> r2 r1 . ((weak_previous (\<lambda> r4 r3 . (\<not> (trigger r3))) r2 r1) \<or> (constrained_until2 fin (fin + delay) Inv (\<lambda> r4 r3 . ((reaction r4 r3) \<and> (Inv r4 r3))) r2 r1))) s)"
+definition EDTL_trigger_prev_release_false_final_tau_delay_tau where "EDTL_trigger_prev_release_false_final_tau_delay_tau fin delay trigger Inv reaction s \<equiv> (always (\<lambda> r2 r1 . ((weak_previous (\<lambda> r4 r3 . (\<not> (trigger r3))) r2 r1) \<or> (constrained_until fin (fin + delay) Inv (\<lambda> r4 r3 . ((reaction r4 r3) \<and> (Inv r4 r3))) r2 r1))) s)"
 
 definition EDTL_trigger_prev_release_false_final_tau_delay_tau_part where "EDTL_trigger_prev_release_false_final_tau_delay_tau_part fin delay trigger Inv reaction s \<equiv> (EDTL_trigger_prev_release_false_final_tau_delay_tau fin delay trigger (\<lambda> s s1 . (Inv s1)) (\<lambda> s s1 . (reaction s1)) s)"
 
-definition EDTL_trigger_prev_release_false_final_tau_delay_tau_inv where "EDTL_trigger_prev_release_false_final_tau_delay_tau_inv fin delay b_0 t1_1_0 t2_1_0 trigger Inv_1 reaction_1 s \<equiv> ((always_inv (\<lambda> r2 r1 . ((weak_previous (\<lambda> r4 r3 . (\<not> (trigger r3))) r2 r1) \<or> (constrained_until2_inv fin (fin + delay) t1_1_0 t2_1_0 Inv_1 (\<lambda> r4 r3 . ((reaction_1 r4 r3) \<and> (Inv_1 r4 r3))) r2 r1))) s) \<and> (previous_inv b_0 (\<lambda> r4 r3 . (\<not> (trigger r3))) s))"
+definition EDTL_trigger_prev_release_false_final_tau_delay_tau_inv where "EDTL_trigger_prev_release_false_final_tau_delay_tau_inv fin delay b_0 t1_1_0 t2_1_0 trigger Inv_1 reaction_1 s \<equiv> ((always_inv (\<lambda> r2 r1 . ((weak_previous (\<lambda> r4 r3 . (\<not> (trigger r3))) r2 r1) \<or> (constrained_until_inv fin (fin + delay) t1_1_0 t2_1_0 Inv_1 (\<lambda> r4 r3 . ((reaction_1 r4 r3) \<and> (Inv_1 r4 r3))) r2 r1))) s) \<and> (previous_inv b_0 (\<lambda> r4 r3 . (\<not> (trigger r3))) s))"
 
 definition EDTL_trigger_prev_release_false_final_tau_delay_tau_inv_part where "EDTL_trigger_prev_release_false_final_tau_delay_tau_inv_part fin delay b_0 t1_1_0 t2_1_0 trigger Inv reaction s \<equiv> (EDTL_trigger_prev_release_false_final_tau_delay_tau_inv fin delay b_0 t1_1_0 t2_1_0 trigger (\<lambda> s s1 . (Inv s1)) (\<lambda> s s1 . (reaction s1)) s)"
 
@@ -2638,7 +2691,7 @@ apply(erule conjE)
 subgoal premises prems1
 apply(rule conjI)
 apply(insert prems1(1,2,4))[1]
-apply(erule always_rule)
+apply(erule always_inv_saving_gen)
   apply simp
   apply(erule conjE)
   subgoal premises prems2
@@ -2650,11 +2703,11 @@ apply(erule always_rule)
       subgoal premises prems3
       apply(rule conjI)
       apply(insert prems3(1,2))[1]
-        apply(rule weak_previous_LS4)
+        apply(rule weak_previous_L4)
         apply simp
           apply(rule always_imp_refl)
       apply(insert prems3(1,3))
-        apply(rule constrained_until2_rule)
+        apply(rule constrained_until_L1)
         apply simp
           apply(erule conjE)
           subgoal premises prems4
@@ -2731,7 +2784,7 @@ apply(erule always_rule)
   apply(insert prems2(1,3))
     apply(erule disjE)
     apply(rule disjI1)
-      apply(rule weak_previous_one_point[OF prems1(3)])
+      apply(rule weak_previous_L7[OF prems1(3)])
       apply simp
         apply(erule conjE)
         subgoal premises prems12
@@ -2742,7 +2795,7 @@ apply(erule always_rule)
           apply(rule always_imp_refl)
         done
     apply(rule disjI2)
-      apply(rule constrained_until2_one_point)
+      apply(rule constrained_until_L2)
       apply simp
         apply(erule disjE)
         apply(rule disjI1)
@@ -2779,7 +2832,7 @@ apply(erule always_rule)
           done
   done
 apply(insert prems1(1,3,5))
-  apply(erule previous_rule)
+  apply(erule previous_inv_L6)
   apply simp
   apply(rule impI)
   apply(erule impE)
@@ -2803,7 +2856,7 @@ apply(insert prems1(1,2))
 apply(erule conjE)
 subgoal premises prems2
 apply(insert prems2(1,2) prems1(3))
-apply(erule always_einv2req)
+apply(erule always_einv_imp_req_gen)
 apply simp
   apply(rule always_disj_rule)
   apply simp
@@ -2811,11 +2864,11 @@ apply simp
     subgoal premises prems3
     apply(rule conjI)
     apply(insert prems3(1,2))[1]
-      apply(rule weak_previous_LS5)
+      apply(rule weak_previous_L5)
       apply simp
         apply(rule always_imp_refl)
     apply(insert prems3(1,3))
-      apply(rule constrained_until2_einv2req)
+      apply(rule constrained_until_L3)
       apply simp
         apply(erule conjE)
         subgoal premises prems4
@@ -2868,9 +2921,9 @@ done
 
 
 
-lemmas EDTL_trigger_prev_release_false_final_tau_delay_tau_used_patterns = EDTL_trigger_prev_release_false_final_tau_delay_tau_def always_used_patterns weak_previous_def constrained_until2_def 
+lemmas EDTL_trigger_prev_release_false_final_tau_delay_tau_used_patterns = EDTL_trigger_prev_release_false_final_tau_delay_tau_def always_used_patterns weak_previous_def constrained_until_def 
 
-lemmas EDTL_trigger_prev_release_false_final_tau_delay_tau_inv_used_patterns = EDTL_trigger_prev_release_false_final_tau_delay_tau_inv_def always_inv_used_patterns weak_previous_def constrained_until2_inv_def previous_inv_def 
+lemmas EDTL_trigger_prev_release_false_final_tau_delay_tau_inv_used_patterns = EDTL_trigger_prev_release_false_final_tau_delay_tau_inv_def always_inv_used_patterns weak_previous_def constrained_until_inv_def previous_inv_def 
 
 lemmas EDTL_trigger_prev_release_false_final_tau_delay_tau_inv_part_used_patterns = EDTL_trigger_prev_release_false_final_tau_delay_tau_inv_part_def EDTL_trigger_prev_release_false_final_tau_delay_tau_inv_used_patterns
 
