ROOT
@@ -1,3 +1,2 @@
 session VCProving = HOL +
-  sessions "HOL-Eisbach"
   theories  Basic_Patterns Derived_Patterns EDTL_Patterns
